pcuic/theories/PCUICWfUniverses.v
@@ -36,6 +36,63 @@ Qed.
 Section CheckerFlags.
   Context {cf:checker_flags}.
 
+  Lemma subst_instance_id_mdecl Σ u mdecl :
+    consistent_instance_ext Σ (ind_universes mdecl) u ->
+    subst_instance u (abstract_instance (ind_universes mdecl)) = u.
+  Proof using Type.
+    intros cu.
+    red in cu. red in cu.
+    destruct (ind_universes mdecl) eqn:eqi.
+    - destruct u; simpl in cu; try discriminate.
+      unfold abstract_instance, subst_instance, subst_instance_instance.
+      cbn. destruct cu. apply length_nil in H, H0. rewrite H H0 //.
+    - simpl. destruct cst as [univs csts]. simpl.
+      destruct u. unfold subst_instance, subst_instance_instance. cbn.
+      unfold Instance.make. f_equal; rewrite map_mapi; simpl in *;
+        destruct cu as [Hu [sizeu [sizeq vu]]]; now rewrite mapi_nth.
+  Qed.
+
+  Lemma declared_inductive_wf_ext_wk Σ mdecl mind :
+    wf Σ ->
+    declared_minductive Σ mind mdecl ->
+    wf_ext_wk (Σ, ind_universes mdecl).
+  Proof using Type.
+    intros wfΣ decli. eapply declared_minductive_to_gen in decli.
+    epose proof (weaken_lookup_on_global_env' _ _ (InductiveDecl mdecl) wfΣ decli); eauto.
+    red. simpl. split; auto.
+    Unshelve. all:eauto.
+  Qed.
+
+  Lemma declared_inductive_wf_global_ext Σ mdecl mind :
+    wf Σ ->
+    declared_minductive Σ mind mdecl ->
+    wf_global_ext Σ (ind_universes mdecl).
+  Proof using Type.
+    intros wfΣ decli. eapply declared_minductive_to_gen in decli.
+    split; auto.
+    epose proof (weaken_lookup_on_global_env' _ _ (InductiveDecl mdecl) wfΣ decli); eauto.
+    Unshelve. all:eauto.
+  Qed.
+
+  Lemma udecl_prop_in_var_poly {Σ : global_env_ext} {n} :
+    LevelSet.In (Level.lvar n) (levels_of_udecl Σ.2) ->
+    ∑ ctx, Σ.2 = Polymorphic_ctx ctx.
+  Proof using Type. clear cf.
+    intros lin.
+    destruct (Σ.2); intuition eauto.
+    simpl in lin. lsets.
+  Qed.
+
+  Lemma udecl_in_var_quality_poly {Σ : global_env_ext} {n} :
+    QualitySet.In (Quality.var n) (qualities_of_udecl Σ.2) -> ∑ ctx, Σ.2 = Polymorphic_ctx ctx.
+  Proof using Type. clear cf.
+    intros lin. destruct (Σ.2); intuition eauto.
+    simpl in lin. qsets.
+  Qed.
+
+  Hint Resolve declared_inductive_wf_ext_wk declared_inductive_wf_global_ext : pcuic.
+
+
   Lemma wf_sort_type0 Σ : wf_sort Σ Sort.type0.
   Proof using Type.
     simpl.
@@ -52,35 +109,49 @@ Section CheckerFlags.
     apply global_ext_levels_InSet.
   Qed.
 
-  Lemma wf_sort_super {Σ u} : wf_sort Σ u -> wf_sort Σ (Sort.super u).
-  Proof using Type.
-    destruct u; cbn.
-    1-2:intros _ l hin%LevelExprSet.singleton_spec; subst l; apply wf_sort_type1;
-     now apply LevelExprSet.singleton_spec.
-    intros Hl.
-    intros l hin.
+  Lemma wf_universe_succ {Σ u} : wf_universe Σ u -> wf_universe Σ (Universe.succ u).
+  Proof.
+    intros h l hin.
     eapply Universes.spec_map_succ in hin as [x' [int ->]].
-    simpl. now specialize (Hl _ int).
+    simpl. now specialize (h _ int).
   Qed.
 
-  Lemma wf_sort_sup {Σ u u'} : wf_sort Σ u -> wf_sort Σ u' ->
-    wf_sort Σ (Sort.sup u u').
+  Lemma wf_sort_super {Σ u} : wf_sort Σ u -> wf_sort Σ (Sort.super u).
   Proof using Type.
-    destruct u, u'; cbn; auto.
-    intros Hu Hu' l [Hl|Hl]%LevelExprSet.union_spec.
+    destruct u; cbn => Hu.
+    all: try apply wf_sort_type1.
+    all: apply wf_universe_succ; auto.
+    apply Hu.
+  Qed.
+
+  Lemma wf_universe_sup {Σ l l'} : wf_universe Σ l -> wf_universe Σ l' ->
+    wf_universe Σ (Universe.sup l l').
+  Proof using Type.
+    intros Hu Hu' x [Hl|Hl]%LevelExprSet.union_spec.
     now apply (Hu _ Hl).
     now apply (Hu' _ Hl).
+  Qed.
+
+  Lemma wf_sort_sup {Σ l u} : wf_universe Σ l -> wf_sort Σ u ->
+    wf_universe Σ (Sort.sup l u).
+  Proof using Type.
+    destruct u; cbn; auto using wf_universe_sup.
+    intros ? []; by apply wf_universe_sup.
   Qed.
 
   Lemma wf_sort_product {Σ s s'} : wf_sort Σ s -> wf_sort Σ s' ->
     wf_sort Σ (Sort.sort_of_product s s').
   Proof using Type.
-    intros Hu Hu'.
-    destruct s' => //=.
-    now apply wf_sort_sup.
+    destruct s' => //= Hu Hu'.
+    - now apply wf_sort_sup.
+    - destruct Hu'. split; tas.
+      now apply wf_sort_sup.
   Qed.
 
-  Hint Resolve wf_sort_type1 wf_sort_super wf_sort_sup wf_sort_product : pcuic.
+  Hint Resolve wf_sort_type1 wf_sort_super wf_sort_product : pcuic.
+
+  Definition wf_qvarb Σ qv :=
+    QualitySet.mem (Quality.qVar qv) (global_ext_qualities Σ).
 
   Definition wf_qualityb Σ q :=
     QualitySet.mem q (global_ext_qualities Σ).
@@ -109,6 +180,11 @@ Section CheckerFlags.
     now apply QualitySet.mem_spec in e.
     intros hin.
     now apply QualitySet.mem_spec in hin.
+  Qed.
+
+  Lemma wf_qvarP {Σ qv} : reflect (wf_qvar Σ qv) (wf_qvarb Σ qv).
+  Proof using Type.
+    apply wf_qualityP.
   Qed.
 
   Lemma wf_levelP {Σ l} : reflect (wf_level Σ l) (wf_levelb Σ l).
@@ -158,14 +234,33 @@ Section CheckerFlags.
       + now apply not_var_global_levels in Hl.
   Qed.
 
+  Lemma wf_quality_subst_instance_qvar (Σ : global_env_ext) univs ui qv :
+    wf Σ ->
+    wf_instance (Σ.1, univs) ui ->
+    wf_quality (Σ.1, univs) (subst_instance_qvar ui qv).
+  Proof using Type.
+    intros wfΣ [Hq _].
+    destruct qv; cbnr.
+    rewrite nth_nth_error.
+    destruct nth_error eqn:hnth.
+    - eapply nth_error_forall in Hq; tea.
+    - global_ext_qconst_InSet.
+  Qed.
+
   Lemma wf_sort_subst_instance_sort (Σ : global_env_ext) univs u s :
     wf Σ ->
     wf_sort Σ s ->
     wf_instance (Σ.1, univs) u ->
     wf_sort (Σ.1, univs) (subst_instance u s).
   Proof using Type.
-    destruct s as [| |t]; cbnr.
-    apply wf_universe_subst_instance_univ.
+    destruct s; cbnr.
+    - apply wf_universe_subst_instance_univ.
+    - intros ? [] ?.
+      eapply wf_quality_subst_instance_qvar with (qv := t) in H1 as Hq; tea.
+      destruct subst_instance_qvar; cbnr.
+      + now apply wf_universe_subst_instance_univ.
+      + split; tas.
+        now apply wf_universe_subst_instance_univ.
   Qed.
 
   Lemma wf_sort_instantiate Σ univs s u φ :
@@ -212,7 +307,7 @@ Section CheckerFlags.
     induction 1 => /= //.
     destruct x eqn:isv => /= //.
     apply LS.union_spec in H as [H|H]; simpl in H.
-    epose proof (@udecl_prop_in_var_poly _ (Σ, _) _ uprop H) as [ctx' eq].
+    epose proof (@udecl_prop_in_var_poly (Σ, Monomorphic_ctx) _ H) as [ctx' eq].
     discriminate.
     now pose proof (not_var_global_levels wf _ H).
   Qed.
@@ -299,7 +394,7 @@ Section CheckerFlags.
       * have Hin: In t (Instance.qualities u) by now eapply nth_error_In.
         eapply Forall_In in Hq; eauto.
       * now apply QualitySetProp.FM.add_1.
-    - unfold wf_quality in Hq |- *. rewrite nth_nth_error.
+    - unfold wf_quality in Hq |- *. cbn. rewrite nth_nth_error.
       destruct (nth_error (Instance.qualities u) n) eqn:e; global_ext_qconst_InSet.
       eapply Forall_In in Hq; eauto. now eapply nth_error_In.
   Qed.
@@ -331,7 +426,7 @@ Section CheckerFlags.
         unfold AUContext.levels, AUContext.repr in wfx.
         destruct cst as [? cst]. cbn in wfx.
         eapply (proj1 (LevelSetProp.of_list_1 _ _)) in wfx.
-        rewrite mapi_unfold in wfx. 
+        rewrite mapi_unfold in wfx.
         apply SetoidList.InA_alt in wfx as [? [<- wfx]]. simpl in wfx.
         eapply In_unfold_inj in wfx; [|congruence].
         destruct (nth_in_or_default n (Instance.universes u) (Level.lzero)).
@@ -383,42 +478,98 @@ Section CheckerFlags.
            eapply nth_error_In; eauto.
     Qed.
 
+    Definition on_binder_annot fq (na : aname) :=
+      on_relevance fq true na.(binder_relevance).
+
+    Definition on_instance fq fu ui :=
+      forallb fq (Instance.qualities ui) &&
+      forallb fu (map Universe.make' (Instance.universes ui)).
+
+    Definition on_decl_universes (ft : term -> bool) (fq : Quality.t -> bool) (fu : Universe.t -> bool) d :=
+      on_binder_annot (fq ∘ Quality.qVar) d.(decl_name) &&
+      option_default ft d.(decl_body) true &&
+      ft d.(decl_type).
+
+    Definition on_ctx_universes (ft : term -> bool) (fq : Quality.t -> bool) (fu : Universe.t -> bool) Γ :=
+      forallb (on_decl_universes ft fq fu) Γ.
+
     Fixpoint on_universes fq fu fc t :=
       match t with
-      | tSort s => Sort.on_sort fu true s
-      | tApp t u
-      | tProd _ t u
-      | tLambda _ t u => on_universes fq fu fc t && on_universes fq fu fc u
-      | tCase _ p c brs =>
+      | tSort s => Sort.on_sort (fq ∘ Quality.qVar) fu true andb s
+      | tApp t u => on_universes fq fu fc t && on_universes fq fu fc u
+      | tProd na t u
+      | tLambda na t u => on_binder_annot (fq ∘ Quality.qVar) na && on_universes fq fu fc t && on_universes fq fu fc u
+      | tCase ci p c brs =>
         [&&
-        forallb fu (map Universe.make' (Instance.universes p.(puinst))),
-        forallb fq (Instance.qualities p.(puinst)),
+        on_relevance (fq ∘ Quality.qVar) true ci.(ci_relevance),
+        on_instance fq fu p.(puinst),
         forallb (on_universes fq fu fc) p.(pparams) ,
-        test_context (fc #|Instance.universes p.(puinst)|) p.(pcontext) ,
+        fc p.(puinst) p.(pcontext),
         on_universes fq fu fc p.(preturn) ,
         on_universes fq fu fc c &
-        forallb (test_branch (fc #|Instance.universes p.(puinst)|) (on_universes fq fu fc)) brs]
-      | tLetIn _ t t' u =>
-        [&& on_universes fq fu fc t , on_universes fq fu fc t' & on_universes fq fu fc u]
+        forallb (fun br => fc p.(puinst) br.(bcontext) && on_universes fq fu fc br.(bbody)) brs]
+      | tLetIn na t t' u =>
+        [&& on_binder_annot (fq ∘ Quality.qVar) na,
+          on_universes fq fu fc t , on_universes fq fu fc t' & on_universes fq fu fc u]
       | tProj _ t => on_universes fq fu fc t
       | tFix mfix _ | tCoFix mfix _ =>
-        forallb (fun d => on_universes fq fu fc d.(dtype) && on_universes fq fu fc d.(dbody)) mfix
+        forallb (fun d => on_binder_annot (fq ∘ Quality.qVar) d.(dname) && on_universes fq fu fc d.(dtype) && on_universes fq fu fc d.(dbody)) mfix
       | tConst _ u | tInd _ u | tConstruct _ _ u =>
-          forallb fu (map Universe.make' (Instance.universes u)) &&
-            forallb fq (Instance.qualities u)
+        on_instance fq fu u
       | tEvar _ args => forallb (on_universes fq fu fc) args
       | tPrim p => test_primu (fun x => fu (Universe.make' x)) (on_universes fq fu fc) p
       | _ => true
       end.
 
-    Definition wf_universes t := on_universes (wf_qualityb Σ) wf_universeb closedu t.
-    Definition wf_sortb s := Sort.on_sort wf_universeb true s.
+    Definition wf_ctx_inner u :=
+      let q := #|Instance.qualities u| in let u := #|Instance.universes u| in
+      on_ctx_universes (fun t => closedq q t && closedu u t) (closedq_quality q) (closedu_universe u).
+
+    Definition wf_universes t := on_universes (wf_qualityb Σ) wf_universeb wf_ctx_inner t.
+    Definition wf_sortb s := Sort.on_sort (wf_qvarb Σ) wf_universeb true andb s.
+    Definition wf_relb r := on_relevance (wf_qvarb Σ) true r.
+    Definition wf_anameb na := on_binder_annot (wf_qvarb Σ) na.
+
+    Definition wf_decl_universes := on_decl_universes wf_universes (wf_qualityb Σ) wf_universeb.
+    Definition wf_ctx_universes := forallb wf_decl_universes.
+
+    Lemma on_instance_reflect ui :
+      reflect (wf_instance Σ ui) (on_instance (wf_qualityb Σ) wf_universeb ui).
+    Proof.
+      unfold on_instance. rewrite forallb_map.
+      apply andPP; apply forallbP => x.
+    - apply wf_qualityP.
+    - apply iff_reflect.
+      rewrite -/(is_true _) -(rwP wf_universe_reflect).
+      split.
+      + intros H x' Hin.
+        unfold Universe.make' in Hin.
+        apply LevelExprSet.singleton_spec in Hin as ->. cbn. assumption.
+      + move/(_ (LevelExpr.make x)).
+        apply. by apply LevelExprSet.singleton_spec.
+    Qed.
 
     Lemma wf_sort_reflect {s : sort} :
       reflect (wf_sort Σ s) (wf_sortb s).
     Proof using Type.
       destruct s => //=; repeat constructor.
-      apply wf_universe_reflect.
+      - apply wf_universe_reflect.
+      - apply andPP.
+        + apply wf_qvarP.
+        + apply wf_universe_reflect.
+    Qed.
+
+    Lemma on_relevance_reflect r :
+      reflect (wf_relevance Σ r) (on_relevance (wf_qvarb Σ) true r).
+    Proof.
+      destruct r => //=; try by constructor.
+      apply wf_qvarP.
+    Qed.
+
+    Lemma on_binder_annot_reflect na :
+      reflect (wf_aname Σ na) (on_binder_annot (wf_qvarb Σ) na).
+    Proof.
+      apply on_relevance_reflect.
     Qed.
 
     Lemma wf_universeb_instance_forall u :
@@ -429,6 +580,26 @@ Section CheckerFlags.
       f_equal.
       cbn.
       now rewrite if_true_false.
+    Qed.
+
+    Lemma wf_relevance_subst_instance u r :
+      wf Σ ->
+      wf_instance Σ u ->
+      wf_relevance Σ (subst_instance u r).
+    Proof.
+      intros wfΣ wfui.
+      destruct r => //=.
+      eapply wf_quality_subst_instance_qvar with (qv := t) in wfui; tea.
+      cbn. destruct subst_instance_qvar => //.
+    Qed.
+
+    Lemma wf_aname_subst_instance u na :
+      wf Σ ->
+      wf_instance Σ u ->
+      wf_aname Σ (subst_instance u na).
+    Proof.
+      intros wfΣ wfui.
+      by apply wf_relevance_subst_instance.
     Qed.
 
     (* Lemma All_forallb {A} (P : A -> Type) l (H : All P l) p p' : (forall x, P x -> p x = p' x) -> forallb p l = forallb p' l.
@@ -530,10 +701,16 @@ Section CheckerFlags.
     | [ |- is_true (wf_qualityb _ ?x) ] => apply (introT (@wf_qualityP _ x))
     | [ H: is_true (wf_universeb _ ?x) |- _ ] => apply (elimT (@wf_universe_reflect _ x)) in H
     | [ |- is_true (wf_universeb _ ?x) ] => apply (introT (@wf_universe_reflect _ x))
-    | [ H: is_true (Sort.on_sort (wf_universeb _) _ ?x) |- _ ] => apply (elimT (@wf_sort_reflect _ x)) in H
-    | [ |- is_true (Sort.on_sort (wf_universeb _) _ ?x) ] => apply (introT (@wf_sort_reflect _ x))
+    | [ H: is_true (Sort.on_sort _ (wf_universeb _) _ _ ?x) |- _ ] => apply (elimT (@wf_sort_reflect _ x)) in H
+    | [ |- is_true (Sort.on_sort _ (wf_universeb _) _ _ ?x) ] => apply (introT (@wf_sort_reflect _ x))
     | [ H: is_true (wf_sortb _ ?x) |- _ ] => apply (elimT (@wf_sort_reflect _ x)) in H
     | [ |- is_true (wf_sortb _ ?x) ] => apply (introT (@wf_sort_reflect _ x))
+    | [ H: is_true (on_instance (wf_qualityb _) (wf_universeb _) ?x) |- _ ] => apply (elimT (@on_instance_reflect _ x)) in H
+    | [ |- is_true (on_instance (wf_qualityb _) (wf_universeb _) ?x) ] => apply (introT (@on_instance_reflect _ x))
+    | [ H: is_true (on_relevance _ _ ?x) |- _ ] => apply (elimT (@on_relevance_reflect _ x)) in H
+    | [ |- is_true (on_relevance _ _ ?x) ] => apply (introT (@on_relevance_reflect _ x))
+    | [ H: is_true (on_binder_annot _ ?x) |- _ ] => apply (elimT (@on_binder_annot_reflect _ x)) in H
+    | [ |- is_true (on_binder_annot _ ?x) ] => apply (introT (@on_binder_annot_reflect _ x))
     end.
 
   Lemma wf_universes_inst {Σ : global_env_ext} univs t u :
@@ -544,25 +721,21 @@ Section CheckerFlags.
     wf_universes Σ (subst_instance u t).
   Proof using Type.
     intros wfΣ onudecl cu wft.
-    induction t using term_forall_list_ind; simpl in *; auto; try to_prop;
-      try apply /andP; intuition eauto 4.
-
-    all:cbn -[Universe.make'] in * ; to_wfu; autorewrite with map; repeat (f_equal; solve_all).
-
-    - destruct Σ as [Σ univs']. simpl in *.
-      eapply (wf_sort_subst_instance_sort (Σ, univs)); auto.
-    - to_wfu. eapply wf_universe_subst_instance; eauto.
-    - to_wfu. eapply wf_quality_subst_instance; eauto.
-    - to_wfu. eapply wf_universe_subst_instance; eauto.
-    - to_wfu. eapply wf_quality_subst_instance; eauto.
-    - to_wfu. eapply wf_universe_subst_instance; eauto.
-    - to_wfu. eapply wf_quality_subst_instance; eauto.
-    - to_wfu. eapply wf_universe_subst_instance; eauto.
-    - to_wfu. eapply wf_quality_subst_instance; eauto.
-    - rewrite /test_branch. rtoProp.
-      move/andP: a => [] tctx wfu.
-      split; auto.
-    - rewrite -subst_instance_universe_make. to_wfu.
+    induction t using term_forall_list_ind.
+    all: simpl in *; auto.
+    all: cbn -[Universe.make' wf_qualityb] in *.
+    all: to_prop.
+    all: rtoProp; repeat match goal with |- _ /\ _ => apply conj end.
+    all: to_wfu; eauto using wf_instance_subst_instance, wf_sort_instantiate, wf_relevance_subst_instance, wf_aname_subst_instance.
+    all: try solve [ solve_all;
+      to_wfu;
+      eauto using wf_aname_subst_instance
+    ].
+    - rewrite !length_map //.
+    - solve_all.
+      rewrite /wf_ctx_inner !length_map //.
+    - solve_all.
+      rewrite -subst_instance_universe_make. to_wfu.
       eapply (wf_universe_subst_instance_univ (Σ.1, univs)) => //.
   Qed.
 
@@ -575,6 +748,26 @@ Section CheckerFlags.
     apply LS.union_spec. apply LS.union_spec in Hl as [Hl|Hl]; simpl.
     left; auto.
     right. now eapply global_levels_sub; [apply ext|].
+  Qed.
+
+  Lemma weaken_wf_quality Σ Σ' t : wf Σ' -> extends Σ.1 Σ' ->
+    wf_quality Σ t ->
+    wf_quality (Σ', Σ.2) t.
+  Proof using Type.
+    intros wfΣ ext Hl.
+    apply QualitySet.union_spec.
+    apply QualitySet.union_spec in Hl as [Hl|Hl]; eauto.
+  Qed.
+
+  Lemma weaken_wf_sort Σ Σ' t : wf Σ' -> extends Σ.1 Σ' ->
+    wf_sort Σ t ->
+    wf_sort (Σ', Σ.2) t.
+  Proof using Type.
+    destruct t => //=.
+    - apply weaken_wf_universe.
+    - intros ??[]; split.
+      + by apply weaken_wf_quality.
+      + by apply weaken_wf_universe.
   Qed.
 
   Lemma weaken_wf_level {Σ : global_env_ext} Σ' t : wf Σ -> wf Σ' -> extends Σ Σ' ->
@@ -620,25 +813,22 @@ Section CheckerFlags.
     wf_universes Σ t ->
     wf_universes (Σ', Σ.2) t.
   Proof using Type.
-    intros wfΣ wfΣ' ext.
-    induction t using term_forall_list_ind; cbn in *; auto; intros; to_prop;
-    try apply /andP; to_wfu; intuition eauto 4.
-
-  - solve_all.
-  - move: H. destruct s => //=.
-    now apply weaken_wf_universe.
-  - eapply forallb_impl ; tea.
-    now move => ? _ /wf_universe_reflect /weaken_wf_universe /wf_universe_reflect.
-  - eapply forallb_impl ; tea.
-    now move => ? _ /wf_universe_reflect /weaken_wf_universe /wf_universe_reflect.
-  - eapply forallb_impl ; tea.
-    now move => ? _ /wf_universe_reflect /weaken_wf_universe /wf_universe_reflect.
-  - eapply forallb_impl ; tea.
-    now move => ? _ /wf_universe_reflect /weaken_wf_universe /wf_universe_reflect.
-  - red in X.
-    solve_all; rewrite /test_branch in b |- *; rtoProp; intuition.
-  - red in X; solve_all.
-  - red in X. solve_all.
+    intros wfΣ wfΣ' ext wft.
+    induction t using term_forall_list_ind.
+    all: simpl in *; auto.
+    all: cbn -[Universe.make' wf_qualityb] in *.
+    all: to_prop.
+    all: rtoProp; repeat match goal with |- _ /\ _ => apply conj end.
+    all: to_wfu; eauto.
+    all: try solve [ solve_all ].
+  - rewrite -/(wf_sortb _ s) in wft.
+    rewrite -/(wf_sortb _ s).
+    to_wfu.
+    now apply weaken_wf_sort.
+  - eapply weaken_wf_instance ; tea.
+  - eapply weaken_wf_instance ; tea.
+  - eapply weaken_wf_instance ; tea.
+  - eapply weaken_wf_instance ; tea.
   - eapply test_primu_test_primu_tPrimProp; tea; cbn; eauto.
     intros; to_wfu; now eapply weaken_wf_universe.
   Qed.
@@ -653,13 +843,14 @@ Section CheckerFlags.
 
   Lemma wf_universes_weaken :
     weaken_env_prop cumulSpec0 (lift_typing typing)
-      (fun Σ _ j => option_default (wf_universes Σ) (j_term j) true && wf_universes Σ (j_typ j) && option_default (wf_sortb Σ) (j_univ j) true).
+      (fun Σ _ j => lift_wfbu_term (wf_universes Σ) (wf_sortb Σ) (wf_relb Σ) j).
   Proof using Type.
     intros Σ Σ' φ wfΣ wfΣ' Hext _ j Hj.
     pose proof (fun t => @weaken_wf_universes (Σ, φ) Σ' t wfΣ wfΣ' Hext).
+    unfold lift_wfbu_term in *.
     rtoProp; repeat split; auto.
-    1: destruct j_term => //; cbn in *; auto.
-    1: destruct j_univ => //; cbn in *; now apply (H (tSort _)).
+    + destruct j_term => //; cbn in *; auto.
+    + destruct j_univ => //; cbn in *; now apply (H (tSort _)).
   Qed.
 
   Lemma wf_universes_inds Σ mind u bodies :
@@ -671,10 +862,7 @@ Section CheckerFlags.
     generalize #|bodies|.
     induction n; simpl; auto.
     constructor; auto.
-    cbn.
-    rewrite wf_universeb_instance_forall.
-    apply (introT (@wf_instanceP _ u)) in wfi. rewrite andb_and in wfi.
-    now destruct wfi.
+    cbn. by to_wfu.
   Qed.
 
   Lemma wf_universes_mkApps Σ f args :
@@ -708,9 +896,9 @@ Section CheckerFlags.
     end.
 
   Local Lemma wf_universes_local_ctx_smash (Σ : global_env_ext) mdecl args sorts :
-    sorts_local_ctx (fun Σ _ => lift_wfbu_term (fun t => wf_universes Σ t) (wf_sortb Σ))
+    sorts_local_ctx (fun Σ _ => lift_wfbu_term (fun t => wf_universes Σ t) (wf_sortb Σ) (wf_relb Σ))
       (Σ.1, ind_universes mdecl) (arities_context (ind_bodies mdecl),,, ind_params mdecl) args sorts ->
-    sorts_local_ctx (fun Σ _ => lift_wfbu_term (fun t => wf_universes Σ t) (wf_sortb Σ))
+    sorts_local_ctx (fun Σ _ => lift_wfbu_term (fun t => wf_universes Σ t) (wf_sortb Σ) (wf_relb Σ))
       (Σ.1, ind_universes mdecl) (arities_context (ind_bodies mdecl),,, ind_params mdecl) (smash_context [] args) sorts.
   Proof using Type.
     induction args as [|[na [b|] ty] args] in sorts |- *; simpl; auto.
@@ -719,65 +907,33 @@ Section CheckerFlags.
     destruct sorts as [|u]; auto.
     intros [X Hj].
     rewrite smash_context_acc /=. split. eauto.
-    apply lift_wfbu_term_f_impl with (f := fun t => _ (_ t)) (1 := Hj) (fu := id) => // t Ht.
+    apply lift_wfbu_term_f_impl with (f := fun t => _ (_ t)) (1 := Hj) (fu := id) (fr := id) => // t Ht.
     rewrite wf_universes_subst.
     clear -X. generalize 0.
     induction args as [|[na [b|] ty] args] in sorts, X |- *; simpl in *; auto.
     - destruct X as [? Hj].
       constructor; eauto.
       rewrite wf_universes_subst. eapply IHargs; eauto.
-      move: Hj => /andP[] /andP[] /= Htm _ _.
+      move: Hj => /andP[] /andP[] /andP[] /= Htm _ _ _.
       now rewrite wf_universes_lift.
     - destruct sorts => //. destruct X.
       constructor => //. eapply IHargs; eauto.
     - now rewrite wf_universes_lift.
   Qed.
 
-  Lemma wf_universes_local_ctx_nth_error Σ P Pu Γ Δ s n d :
-    sorts_local_ctx (fun Σ _ => lift_wfbu_term (P Σ) (Pu Σ)) Σ Γ Δ s ->
+  Lemma wf_universes_local_ctx_nth_error Σ P Pu Pr Γ Δ s n d :
+    sorts_local_ctx (fun Σ _ => lift_wfbu_term (P Σ) (Pu Σ) (Pr Σ)) Σ Γ Δ s ->
     nth_error Δ n = Some d ->
     P Σ (decl_type d).
   Proof using Type.
     induction Δ as [|[na [b|] ty] Δ] in n, s |- *; simpl; auto.
     - now rewrite nth_error_nil.
-    - move => [] h /andP[] /andP[] _ h' _.
+    - move => [] h /andP[] /andP[] /andP[] _ h' _ _.
       destruct n. simpl. move=> [= <-] //=.
       now simpl; eapply IHΔ.
-    - destruct s => //. move => [] h /andP[] /andP[] _ h' _.
+    - destruct s => //. move => [] h /andP[] /andP[] /andP[] _ h' _ _.
       destruct n. simpl. move=> [= <-] //=.
       now simpl; eapply IHΔ.
-  Qed.
-
-  Lemma In_unfold_qvar x n : In x (unfold n Quality.var) <-> exists k, k < n /\ (x = Quality.var k).
-  Proof using Type.
-    split.
-    - induction n => /= //.
-      intros [hin|hin]%in_app_or.
-      destruct (IHn hin) as [k [lt eq]].
-      exists k; auto.
-      destruct hin => //. subst x.
-      eexists; eauto.
-    - intros [k [lt ->]].
-      induction n in k, lt |- *. lia.
-      simpl. apply in_or_app.
-      destruct (lt_dec k n). left; auto.
-      right. left. f_equal. lia.
-  Qed.
-
-  Lemma In_unfold_var x n : In x (unfold n Level.lvar) <-> exists k, k < n /\ (x = Level.lvar k).
-  Proof using Type.
-    split.
-    - induction n => /= //.
-      intros [hin|hin]%in_app_or.
-      destruct (IHn hin) as [k [lt eq]].
-      exists k; auto.
-      destruct hin => //. subst x.
-      eexists; eauto.
-    - intros [k [lt ->]].
-      induction n in k, lt |- *. lia.
-      simpl. apply in_or_app.
-      destruct (lt_dec k n). left; auto.
-      right. left. f_equal. lia.
   Qed.
 
   Lemma wf_abstract_instance Σ decl :
@@ -785,33 +941,22 @@ Section CheckerFlags.
   Proof using Type.
     destruct decl as [|[u cst]]=> /=.
     split; cbn; apply Forall_nil.
-    red. split; cbn; rewrite mapi_unfold; eapply In_Forall.
-    - intros q hin. eapply In_unfold_qvar in hin as [k [lt eq]].
-      subst q. red. eapply QualitySet.union_spec; left. simpl.
+    red. split; cbn; rewrite mapi_unfold; eapply All_Forall, All_unfold.
+    - intros q hin.
+      red. eapply QualitySet.union_spec; left. simpl.
       rewrite /AUContext.qualities /= mapi_unfold.
-      eapply (proj2 (QualitySetProp.of_list_1 _ _)).
-      apply SetoidList.InA_alt. eexists; split; eauto.
-      eapply In_unfold_qvar. exists k; split; eauto.
-    - intros x hin. eapply In_unfold_var in hin as [k [lt eq]].
-      subst x. red.
-      eapply LS.union_spec; left. simpl.
+      eapply QualitySetProp.of_list_1.
+      apply SetoidList.InA_alt.
+      exists (Quality.var q); split; cbnr.
+      apply In_unfold; eauto.
+    - intros l hin.
+      red. eapply LS.union_spec; left. simpl.
       rewrite /AUContext.levels /= mapi_unfold.
-      eapply (proj2 (LevelSetProp.of_list_1 _ _)).
-      apply SetoidList.InA_alt. eexists; split; eauto.
-      eapply In_unfold_var. exists k; split; eauto.
+      eapply LevelSetProp.of_list_1.
+      apply SetoidList.InA_alt.
+      exists (Level.lvar l); split; cbnr.
+      apply In_unfold; eauto.
   Qed.
-
-  Definition on_decl_universes (fq : Quality.t -> bool) (fu : Universe.t -> bool) (fc : nat -> term -> bool) d :=
-      option_default (on_universes fq fu fc) d.(decl_body) true &&
-      on_universes fq fu fc d.(decl_type).
-
-  Definition wf_decl_universes Σ := on_decl_universes (wf_qualityb Σ) (wf_universeb Σ) closedu.
-
-  Definition on_ctx_universes (fq : Quality.t -> bool) (fu : Universe.t -> bool) (fc : nat -> term -> bool) Γ :=
-    forallb (on_decl_universes fq fu fc) Γ.
-
-  Definition wf_ctx_universes Σ Γ :=
-    forallb (wf_decl_universes Σ) Γ.
 
   Lemma wf_universes_it_mkProd_or_LetIn {Σ Γ T} :
     wf_universes Σ (it_mkProd_or_LetIn Γ T) = wf_ctx_universes Σ Γ && wf_universes Σ T.
@@ -819,17 +964,18 @@ Section CheckerFlags.
     induction Γ as [ |[na [b|] ty] Γ] using rev_ind ; simpl; auto;
     rewrite it_mkProd_or_LetIn_app {1}/wf_universes /=
     -!/(wf_universes _ _) IHΓ /wf_ctx_universes forallb_app /=
-    {3}/wf_decl_universes -!/(wf_universes _ _) / on_decl_universes /= /wf_universes;
+    {3}/wf_decl_universes -!/(wf_universes _ _) / on_decl_universes /= /wf_universes ?andb_true_r;
     repeat bool_congr.
 
   Qed.
 
   Lemma wf_universes_it_mkLambda_or_LetIn {Σ Γ T} :
-    wf_universes Σ (it_mkLambda_or_LetIn Γ T) = test_context (wf_universes Σ) Γ && wf_universes Σ T.
+    wf_universes Σ (it_mkLambda_or_LetIn Γ T) = wf_ctx_universes Σ Γ && wf_universes Σ T.
   Proof using Type.
     induction Γ as [ |[na [b|] ty] Γ] using rev_ind; simpl; auto;
-    now rewrite it_mkLambda_or_LetIn_app {1}/wf_universes
-      /= -!/(wf_universes _ _) IHΓ test_context_app /= /test_decl /= ;
+    now rewrite it_mkLambda_or_LetIn_app {1}/wf_universes /=
+    -!/(wf_universes _ _) IHΓ /wf_ctx_universes forallb_app /=
+    {3}/wf_decl_universes -!/(wf_universes _ _) / on_decl_universes /= /wf_universes ?andb_true_r;
     repeat bool_congr.
   Qed.
 
@@ -844,11 +990,11 @@ Section CheckerFlags.
     All (fun t : term => wf_universes Σ t) (extended_subst Γ n).
   Proof using Type.
     induction Γ as [|[na [b|] ty] Γ] in n |- *; simpl; auto.
-    move=> /andP []; rewrite /wf_decl_universes /= => /andP [] wfb wfty wfΓ.
-    constructor; eauto. rewrite wf_universes_subst //. now apply IHΓ.
-    now rewrite wf_universes_lift. eauto.
-    move=> /andP []; rewrite /wf_decl_universes /= => wfty wfΓ.
-    constructor; eauto.
+    - rewrite /wf_decl_universes/on_decl_universes /= => /andP[]/andP[]/andP[] wfna wfb wfty wfΓ.
+      constructor; eauto. rewrite wf_universes_subst //. 1:now apply IHΓ.
+      now rewrite wf_universes_lift.
+    - rewrite /wf_decl_universes/on_decl_universes /= => /andP[]/andP[]wfna wfty wfΓ.
+      constructor; eauto.
   Qed.
 
   Lemma closedu_compare_decls k Γ Δ :
@@ -859,14 +1005,46 @@ Section CheckerFlags.
     f_equal; auto. destruct r; subst; auto.
   Qed.
 
+  Lemma wf_ctx_inner_compare_decls ui Γ Δ :
+    PCUICEquality.eq_context_upto_names Γ Δ ->
+    wf_ctx_inner ui Γ = wf_ctx_inner ui Δ.
+  Proof using Type.
+    induction 1; cbn; auto.
+    f_equal; auto. unfold on_decl_universes, on_binder_annot.
+    destruct r; subst; cbn; auto.
+    all: destruct e; auto.
+  Qed.
+
+  Lemma wf_ctx_inner_lengths ui ui' Γ :
+    #|Instance.qualities ui| = #|Instance.qualities ui'| ->
+    #|Instance.universes ui| = #|Instance.universes ui'| ->
+    wf_ctx_inner ui Γ = wf_ctx_inner ui' Γ.
+  Proof using Type.
+    unfold wf_ctx_inner.
+    by intros <- <-.
+  Qed.
+
+  Lemma closedq_mkApps k f args : closedq k (mkApps f args) = closedq k f && forallb (closedq k) args.
+  Proof using Type.
+    induction args in f |- *; cbn; auto. ring.
+    rewrite IHargs /=. ring.
+  Qed.
+
   Lemma closedu_mkApps k f args : closedu k (mkApps f args) = closedu k f && forallb (closedu k) args.
   Proof using Type.
     induction args in f |- *; cbn; auto. ring.
     rewrite IHargs /=. ring.
   Qed.
 
-  Definition max_length inst := max #|Instance.qualities inst| #|Instance.universes inst|.
-  Definition min_length inst := min #|Instance.qualities inst| #|Instance.universes inst|.
+  Lemma closedq_abstract_instance univs :
+    closed_instance_qualities #|Instance.qualities (abstract_instance univs)|
+    (abstract_instance univs).
+  Proof using Type.
+    destruct univs as [|[l csts]] => // /=.
+    rewrite /UContext.instance /AUContext.repr.
+    rewrite /closed_instance_qualities !forallb_mapi //.
+    intros i hi; cbn; len; now eapply Nat.ltb_lt.
+  Qed.
 
   Lemma closedu_abstract_instance univs :
     closed_instance_universes #|Instance.universes (abstract_instance univs)|
@@ -878,7 +1056,24 @@ Section CheckerFlags.
     intros i hi; cbn; len; now eapply Nat.ltb_lt.
   Qed.
 
+  Notation closedq_ctx_weak k := (test_context (closedq k)).
   Notation closedu_ctx k := (test_context (closedu k)).
+
+  Lemma closedq_lift k n k' t :
+    closedq k (lift n k' t) = closedq k t.
+  Proof using Type.
+    induction t in k' |- * using term_forall_list_ind; cbn; auto; intros; solve_all.
+    - rewrite IHt.
+      rewrite /map_predicate_k /= /test_predicate /test_predicate_kq /= /id.
+      f_equal. f_equal. rewrite e. f_equal. f_equal. f_equal.
+      solve_all.
+      solve_all.
+      all: rewrite /map_branch_k /test_branch /=; f_equal;
+        now rewrite b.
+    - rewrite /test_def/test_def_gen /map_def /=. now rewrite b b0.
+    - rewrite /test_def/test_def_gen /map_def /=. now rewrite b b0.
+    - rewrite !test_primq_test_prim -!test_primu_test_prim test_primu_mapu; eapply test_primu_primProp; tea; eauto.
+  Qed.
 
   Lemma closedu_lift k n k' t :
     closedu k (lift n k' t) = closedu k t.
@@ -891,8 +1086,8 @@ Section CheckerFlags.
       solve_all.
       all: rewrite /map_branch_k /test_branch /=; f_equal;
         now rewrite b.
-    - rewrite /test_def /map_def /=. now rewrite a b.
-    - rewrite /test_def /map_def /=. now rewrite a b.
+    - rewrite /test_def /map_def /=. now rewrite b b0.
+    - rewrite /test_def /map_def /=. now rewrite b b0.
     - rewrite test_primu_mapu; eapply test_primu_primProp; tea; eauto.
   Qed.
 
@@ -900,6 +1095,25 @@ Section CheckerFlags.
     multimatch goal with H : _ |- _ => eapply H end.
 
   Ltac crush := repeat (solve_all; try try_hyp; cbn).
+
+  Lemma closedq_subst k s k' t :
+    forallb (closedq k) s && closedq k t ->
+    closedq k (subst s k' t).
+  Proof using Type.
+    induction t in k' |- * using term_forall_list_ind; cbn; auto; intros;
+      try solve [ repeat (solve_all; try try_hyp) ].
+    - destruct Nat.leb => //.
+      destruct nth_error eqn:eq => //.
+      rtoProp.
+      rewrite closedq_lift.
+      eapply nth_error_forallb in eq; tea.
+    - unfold test_predicate_kq in *. unfold test_branch in *. crush.
+    - unfold test_def, test_def_gen in *; crush.
+    - unfold test_def, test_def_gen in *; crush.
+    - move/andP: H => [].
+      rewrite !test_primq_test_prim -!test_primu_test_prim.
+      crush.
+  Qed.
 
   Lemma closedu_subst k s k' t :
     forallb (closedu k) s && closedu k t ->
@@ -917,6 +1131,26 @@ Section CheckerFlags.
     - unfold test_def in *; crush.
   Qed.
 
+  Lemma wf_ctx_inner_subst_context ui s k Γ :
+    forallb (fun t => closedq #|Instance.qualities ui| t && closedu #|Instance.universes ui| t) s &&
+    wf_ctx_inner ui Γ ->
+    wf_ctx_inner ui (subst_context s k Γ).
+  Proof.
+    rewrite /subst_context.
+    move=> /andP [] Hs.
+    induction Γ.
+    * cbn; auto.
+    * move=> /=/andP[] Ha HΓ. forward IHΓ by assumption.
+      rewrite fold_context_k_snoc0 /= IHΓ // andb_true_r.
+      unfold on_decl_universes, map_decl, map_decl_gen, id in *; cbn -[closedq_quality].
+      rtoProp; split; [split|]; tas.
+      + destruct decl_body; cbnr. cbn in H2.
+        rewrite closedq_subst ?closedu_subst //.
+        all: solve_all.
+      + rewrite closedq_subst ?closedu_subst //.
+        all: solve_all.
+  Qed.
+
   Lemma closedu_subst_context k s k' Γ :
     forallb (closedu k) s && closedu_ctx k Γ ->
     closedu_ctx k (subst_context s k' Γ).
@@ -930,6 +1164,21 @@ Section CheckerFlags.
       destruct decl_body eqn:heq => /= //.
       rewrite closedu_subst //. crush.
       rewrite closedu_subst //. crush.
+  Qed.
+
+  Lemma wf_ctx_inner_lift_context ui n k Γ :
+    wf_ctx_inner ui (lift_context n k Γ) =
+    wf_ctx_inner ui Γ.
+  Proof.
+    unfold lift_context.
+    induction Γ.
+    * cbn; auto.
+    * rewrite /= fold_context_k_snoc0 /=. f_equal; tas.
+      unfold on_decl_universes, map_decl, map_decl_gen, id in *; cbn -[closedq_quality].
+      f_equal. 1:f_equal; tas.
+      + destruct decl_body; cbnr.
+        rewrite closedq_lift closedu_lift //.
+      + rewrite closedq_lift closedu_lift //.
   Qed.
 
   Lemma closedu_lift_context k n k' Γ :
@@ -947,6 +1196,29 @@ Section CheckerFlags.
       rewrite closedu_lift //.
   Qed.
 
+  Lemma closedqu_extended_subst ui Γ k :
+    wf_ctx_inner ui Γ ->
+    forallb (fun t => closedq #|Instance.qualities ui| t && closedu #|Instance.universes ui| t) (extended_subst Γ k).
+  Proof using Type.
+    intro H. move H after k.
+    induction Γ in H, k |- *; cbn; auto.
+    move: H =>/=/andP[] Ha HΓ. forward IHΓ by assumption.
+    unfold on_decl_universes in Ha.
+    destruct a as [na [b|] ty]; cbn in Ha |- *.
+    all: rewrite IHΓ //= andb_true_r.
+    rtoProp; split.
+    - apply closedq_subst.
+      rewrite closedq_lift.
+      rtoProp; split; tas.
+      specialize (IHΓ k).
+      solve_all.
+    - apply closedu_subst.
+      rewrite closedu_lift.
+      rtoProp; split; tas.
+      specialize (IHΓ k).
+      solve_all.
+  Qed.
+
   Lemma closedu_extended_subst k Γ k' :
     closedu_ctx k Γ ->
     forallb (closedu k) (extended_subst Γ k').
@@ -958,6 +1230,16 @@ Section CheckerFlags.
     unfold test_decl; move/andP=> [] clΓ /= cld. now apply IHΓ.
   Qed.
 
+  Lemma wf_ctx_inner_expand_lets_ctx ui Γ Δ :
+    wf_ctx_inner ui Γ && wf_ctx_inner ui Δ ->
+    wf_ctx_inner ui (expand_lets_ctx Γ Δ).
+  Proof using Type.
+    rewrite /expand_lets_ctx /expand_lets_k_ctx.
+    move/andP => [] clΓ clΔ.
+    apply wf_ctx_inner_subst_context.
+    rewrite closedqu_extended_subst // /= wf_ctx_inner_lift_context //.
+  Qed.
+
   Lemma closedu_expand_lets_ctx k Γ Δ :
     closedu_ctx k Γ && closedu_ctx k Δ ->
     closedu_ctx k (expand_lets_ctx Γ Δ).
@@ -966,6 +1248,28 @@ Section CheckerFlags.
     move/andP => [] clΓ clΔ.
     apply closedu_subst_context.
     rewrite closedu_extended_subst // /= closedu_lift_context //.
+  Qed.
+
+  Lemma wf_ctx_inner_smash_context_gen ui Γ Δ :
+    wf_ctx_inner ui Γ -> wf_ctx_inner ui Δ ->
+    wf_ctx_inner ui (smash_context Γ Δ).
+  Proof using Type.
+    induction Δ in Γ |- *; cbn; auto.
+    move=> clΓ /andP[] cla clΔ.
+    destruct a as [na [b|] ty] => //.
+    - apply IHΔ => //.
+      apply wf_ctx_inner_subst_context => /= //.
+      now move: cla => /andP[]/andP[] /= _ -> clty.
+    - apply IHΔ => //.
+      rewrite /wf_ctx_inner/on_ctx_universes forallb_app/=.
+      rtoProp; repeat split; tas.
+  Qed.
+
+  Lemma wf_ctx_inner_smash_context ui Δ :
+    wf_ctx_inner ui Δ ->
+    wf_ctx_inner ui (smash_context [] Δ).
+  Proof using Type.
+    apply wf_ctx_inner_smash_context_gen => //.
   Qed.
 
   Lemma closedu_smash_context_gen k Γ Δ :
@@ -988,21 +1292,31 @@ Section CheckerFlags.
     apply closedu_smash_context_gen => //.
   Qed.
 
-  Lemma wf_quality_closed {Σ : global_env} {wfΣ : wf Σ} univs q :
-    wf_quality (Σ, univs) q -> closedq_quality #|Instance.qualities (polymorphic_instance univs)| q.
+  Lemma wf_qvar_closed {Σ : global_env} univs q :
+    wf_qvar (Σ, univs) q -> closedq_quality #|Instance.qualities (polymorphic_instance univs)| (Quality.qVar q).
   Proof using Type.
-    intros Ht; destruct q => //.
-    unfold closedq_quality. destruct t.
+    intros Ht.
+    unfold closedq_quality. destruct q.
     red in Ht. eapply in_var_global_ext' in Ht => //.
     cbn in Ht. destruct univs. inversion Ht.
     cbn in Ht. unfold AUContext.qualities in Ht.
-    eapply (proj1 (QualitySetProp.of_list_1 _ _)) in Ht.
-    eapply InA_In_eq in Ht. destruct cst as [names cstrs].
+    eapply QualitySetProp.of_list_1 in Ht.
+    eapply SetoidList.InA_alt in Ht.
+    destruct Ht as (q & e & Ht).
+    move:e. destruct q => //=. destruct t => //=. intros <-.
+    destruct cst as [names cstrs].
     unfold AUContext.repr in Ht |- *. cbn in *. len.
-    rewrite mapi_unfold in Ht. eapply In_unfold_qvar in Ht as [k []].
-    injection H0. intros e; rewrite e. eapply Nat.leb_le. assumption.
+    rewrite mapi_unfold in Ht. eapply In_unfold in Ht as [k []].
+    injection H0 as [= <-]. by apply Nat.leb_le.
   Qed.
-  
+
+  Lemma wf_quality_closed {Σ : global_env} univs q :
+    wf_quality (Σ, univs) q -> closedq_quality #|Instance.qualities (polymorphic_instance univs)| q.
+  Proof using Type.
+    intros Ht; destruct q => //.
+    by eapply wf_qvar_closed in Ht.
+  Qed.
+
   Lemma wf_level_closed {Σ : global_env} {wfΣ : wf Σ} univs l :
     on_udecl_prop Σ univs ->
     wf_level (Σ, univs) l -> closedu_level #|Instance.universes (polymorphic_instance univs)| l.
@@ -1012,14 +1326,14 @@ Section CheckerFlags.
     cbn. red in Ht.
     eapply in_var_global_ext in Ht => //.
     cbn in Ht.
-    destruct (udecl_prop_in_var_poly (Σ := (Σ, univs)) ond Ht) as [ctx eq].
+    destruct (udecl_prop_in_var_poly (Σ := (Σ, univs)) Ht) as [ctx eq].
     cbn in eq. subst univs.
     cbn in Ht. cbn. unfold AUContext.levels in Ht.
-    eapply (proj1 (LevelSetProp.of_list_1 _ _)) in Ht.
+    eapply LevelSetProp.of_list_1 in Ht.
     eapply InA_In_eq in Ht.
     destruct ctx as [names cstrs].
     unfold AUContext.repr in Ht |- *. cbn in *. len.
-    rewrite mapi_unfold in Ht. eapply In_unfold_var in Ht as [k []].
+    rewrite mapi_unfold in Ht. eapply In_unfold in Ht as [k []].
     eapply Nat.leb_le. noconf H0. lia.
   Qed.
 
@@ -1038,10 +1352,26 @@ Section CheckerFlags.
 
   Lemma wf_sort_closed {Σ : global_env} {wfΣ : wf Σ} univs s :
     on_udecl_prop Σ univs ->
-    wf_sort (Σ, univs) s -> closedu_sort #|Instance.universes (polymorphic_instance univs)| s.
+    wf_sort (Σ, univs) s ->
+    closedq_sort #|Instance.qualities (polymorphic_instance univs)| s /\
+    closedu_sort #|Instance.universes (polymorphic_instance univs)| s.
   Proof using Type.
     destruct s => //=.
-    apply wf_universe_closed.
+    - split => //; by apply wf_universe_closed.
+    - split.
+      + eapply wf_qvar_closed; apply H0.
+      + by apply wf_universe_closed, H0.
+  Qed.
+
+  Lemma wf_instance_closed {Σ : global_env} {wfΣ : wf Σ} {univs u} :
+    on_udecl_prop Σ univs ->
+    wf_instance (Σ, univs) u ->
+    closed_instance #|Instance.qualities (polymorphic_instance univs)| #|Instance.universes (polymorphic_instance univs)| u.
+  Proof using Type.
+    intros ond [Hq Hu].
+    unfold closed_instance, closed_instance_qualities, closed_instance_universes. solve_all.
+    - now eapply wf_quality_closed; tea.
+    - now apply wf_level_closed.
   Qed.
 
   Lemma wf_instance_universes_closed {Σ : global_env} {wfΣ : wf Σ} {univs u} :
@@ -1052,15 +1382,12 @@ Section CheckerFlags.
     intros Hu. unfold closed_instance_universes. solve_all. apply wf_level_closed; auto.
   Qed.
 
-  Lemma wf_instance_closed {Σ : global_env} {wfΣ : wf Σ} {univs u} :
+  Lemma wf_instance_qualities_closed {Σ : global_env} {wfΣ : wf Σ} {univs u} :
     on_udecl_prop Σ univs ->
-    wf_instance (Σ, univs) u ->
-    closed_instance #|Instance.qualities (polymorphic_instance univs)| #|Instance.universes (polymorphic_instance univs)| u.
+    Forall (wf_quality (Σ, univs)) (Instance.qualities u) ->
+    closed_instance_qualities #|Instance.qualities (polymorphic_instance univs)| u.
   Proof using Type.
-    intros ond [Hq Hu].
-    unfold closed_instance, closed_instance_qualities, closed_instance_universes. solve_all.
-    - now apply wf_quality_closed.
-    - now apply wf_level_closed.
+    intros Hu. unfold closed_instance_qualities. solve_all. eapply wf_quality_closed; tea.
   Qed.
 
   Lemma wf_universe_make Σ u : wf_universe Σ (Universe.make' u) -> wf_level Σ u.
@@ -1069,29 +1396,106 @@ Section CheckerFlags.
     apply (hl (u, 0)). lsets.
   Qed.
 
+  Lemma wf_relevance_closed {Σ : global_env} univs r :
+    wf_relevance (Σ, univs) r -> closedq_rel #|Instance.qualities (polymorphic_instance univs)| r.
+  Proof using Type.
+    unfold wf_relevance, closedq_rel.
+    destruct r => //=.
+    apply wf_qvar_closed.
+  Qed.
+
+  Lemma wf_aname_closed {Σ : global_env} univs na :
+    wf_aname (Σ, univs) na -> closedq_aname #|Instance.qualities (polymorphic_instance univs)| na.
+  Proof using Type.
+    apply wf_relevance_closed.
+  Qed.
+
+  Lemma wf_ctx_inner_closedq ui Γ :
+    wf_ctx_inner ui Γ -> closedq_ctx_weak #|Instance.qualities ui| Γ.
+  Proof.
+    move/forallb_All. induction 1 => //=.
+    unfold on_decl_universes, test_decl in *.
+    rtoProp. split; tas. split; tas.
+    destruct decl_body; cbn in *; by rtoProp.
+  Qed.
+
+  Lemma wf_ctx_inner_closedu ui Γ :
+    wf_ctx_inner ui Γ -> closedu_ctx #|Instance.universes ui| Γ.
+  Proof.
+    move/forallb_All. induction 1 => //=.
+    unfold on_decl_universes, test_decl in *.
+    rtoProp. split; tas. split; tas.
+    destruct decl_body; cbn in *; by rtoProp.
+  Qed.
+
   Lemma wf_universes_closedu {Σ : global_env} {wfΣ : wf Σ} {univs t} :
     on_udecl_prop Σ univs ->
     wf_universes (Σ, univs) t -> closedu #|Instance.universes (polymorphic_instance univs)| t.
   Proof using Type.
-    intros ond. induction t using term_forall_list_ind; cbn => //; solve_all.
-    all: try (apply wf_instance_universes_closed; auto;
-              toAll; eapply All_impl; eauto; intros; apply wf_universe_make).
+    intros ond. induction t using term_forall_list_ind; cbn -[wf_qualityb] => //; solve_all.
+    all: try (toAll; eapply All_impl; eauto; intros; apply wf_universe_make).
     all: try (now move/wf_universe_reflect in H).
-    - apply wf_sort_closed; auto.
-      now move/wf_sort_reflect: H.
+    - to_wfu. apply wf_sort_closed; auto.
+    - to_wfu. apply wf_instance_universes_closed; auto. apply H.
+    - to_wfu. apply wf_instance_universes_closed; auto. apply H.
+    - to_wfu. apply wf_instance_universes_closed; auto. apply H.
     - unfold test_predicate_ku. solve_all.
-      eapply wf_instance_universes_closed => //.
-      apply All_forallb in H0, H.
-      rewrite -forallb_map wf_universeb_instance_forall in H0.
-      have Hinst: wf_instanceb (Σ, univs) (puinst p) by (rewrite andb_and; now split).
-      move/(forallbP (wf_level (Σ, univs)) (wf_levelb (Σ, univs))): H0.
-      intros. apply H0. intros. apply wf_levelP.
+      to_wfu.
+      + by eapply wf_instance_universes_closed, H.
+      + by apply wf_ctx_inner_closedu.
     - unfold test_branch in *; solve_all.
+      by apply wf_ctx_inner_closedu.
     - unfold test_def in *; solve_all.
     - unfold test_def in *; solve_all.
     - eapply test_primu_test_primu_tPrimProp; tea; cbn; eauto.
       intros. to_wfu. apply wf_level_closed; auto.
       now apply wf_universe_make.
+  Qed.
+
+  Lemma wf_universes_closedq {Σ : global_env} {wfΣ : wf Σ} {univs t} :
+    on_udecl_prop Σ univs ->
+    wf_universes (Σ, univs) t -> closedq #|Instance.qualities (polymorphic_instance univs)| t.
+  Proof using Type.
+    intros ond. induction t using term_forall_list_ind; cbn -[wf_qualityb] => //; solve_all.
+    all: try (toAll; eapply All_impl; eauto; intros).
+    all: try (now move/wf_quality_reflect in H).
+    - to_wfu. apply wf_sort_closed; auto.
+    - to_wfu. eapply wf_aname_closed; tea.
+    - to_wfu. eapply wf_aname_closed; tea.
+    - to_wfu. eapply wf_aname_closed; tea.
+    - to_wfu. apply wf_instance_qualities_closed; auto. apply H.
+    - to_wfu. apply wf_instance_qualities_closed; auto. apply H.
+    - to_wfu. apply wf_instance_qualities_closed; auto. apply H.
+    - to_wfu. eapply wf_relevance_closed; tea.
+    - to_wfu. unfold test_predicate_kq. solve_all.
+      + eapply wf_instance_closed in H; tas. unfold closed_instance in H. by rtoProp.
+      + by eapply wf_ctx_inner_closedq.
+    - unfold test_branch in *; solve_all.
+      by eapply wf_ctx_inner_closedq.
+    - unfold test_def, test_def_gen in *; solve_all.
+      to_wfu. eapply wf_aname_closed; tea.
+    - unfold test_def, test_def_gen in *; solve_all.
+      to_wfu. eapply wf_aname_closed; tea.
+    - rewrite test_primq_test_prim -test_primu_test_prim.
+      eapply test_primu_test_primu_tPrimProp; tea; cbn; eauto.
+  Qed.
+
+  Lemma wf_ctx_universes_inner {Σ} {wfΣ : wf Σ} {univs ctx} :
+    on_udecl_prop Σ univs ->
+    wf_ctx_universes (Σ, univs) ctx ->
+    wf_ctx_inner (polymorphic_instance univs) ctx.
+  Proof using Type.
+    intros ond.
+    apply forallb_impl.
+    move => d _ /andP[]/andP[] hna hb hty.
+    to_wfu.
+    apply/andP; split. 1: apply/andP; split.
+    - by apply wf_aname_closed in hna.
+    - destruct decl_body; cbn in *; tas.
+      apply wf_universes_closedq in hb as h1; tas; rewrite h1.
+      apply wf_universes_closedu in hb as h2; tas; rewrite h2.
+    - apply wf_universes_closedq in hty as h1; tas; rewrite h1.
+      apply wf_universes_closedu in hty as h2; tas; rewrite h2.
   Qed.
 
   Lemma wf_ctx_universes_closed {Σ} {wfΣ : wf Σ} {univs ctx} :
@@ -1102,11 +1506,10 @@ Section CheckerFlags.
     intros ond. induction ctx => //.
     rewrite /wf_ctx_universes /= => /andP[] wfa wfctx.
     rewrite IHctx // /=.
-    unfold wf_decl_universes, test_decl in *.
-    destruct a as [na [b|] ty]; cbn in *.
-    move/andP: wfa => [].
-    now do 2 move/(wf_universes_closedu ond) => ->.
-    now move/(wf_universes_closedu ond): wfa => ->.
+    unfold wf_decl_universes, on_decl_universes, test_decl in *.
+    revert wfa. rtoProp.
+    destruct a as [na [b|] ty]; cbn -[wf_qualityb] in *.
+    all: intros [[]]; split => //; eapply wf_universes_closedu; tea.
   Qed.
 
   Lemma closedu_reln k Γ k' acc :
@@ -1127,7 +1530,25 @@ Section CheckerFlags.
     intros clΓ. apply closedu_reln => //.
   Qed.
 
-  Lemma closed_ind_predicate_context {Σ ind mdecl idecl} {wfΣ : wf Σ} :
+  Lemma closedq_reln k Γ k' acc :
+    closedq_ctx_weak k Γ ->
+    forallb (closedq k) acc ->
+    forallb (closedq k) (reln acc k' Γ).
+  Proof using Type.
+    induction Γ in acc, k' |- *; cbn; auto.
+    destruct a as [na [b|] ty] => /= //.
+    - unfold test_decl; move/andP=> [] clΓ /= cld. now eapply IHΓ.
+    - unfold test_decl; move/andP=> [] clΓ /= cld clacc; now apply IHΓ => //.
+  Qed.
+
+  Lemma closedq_to_extended_list_k k Γ k' :
+    closedq_ctx_weak k Γ ->
+    forallb (closedq k) (to_extended_list_k Γ k').
+  Proof using Type.
+    intros clΓ. apply closedq_reln => //.
+  Qed.
+
+  Lemma closedu_ind_predicate_context {Σ ind mdecl idecl} {wfΣ : wf Σ} :
     declared_inductive Σ ind mdecl idecl ->
     closedu_ctx #|Instance.universes (polymorphic_instance (ind_universes mdecl))|
       (ind_params mdecl) ->
@@ -1158,20 +1579,95 @@ Section CheckerFlags.
     eapply closedu_abstract_instance.
   Qed.
 
+  Lemma wf_ctx_subst_inds ind mdecl :
+  forallb (fun t => closedq #|Instance.qualities (abstract_instance (ind_universes mdecl))| t &&
+    closedu #|Instance.universes (abstract_instance (ind_universes mdecl))| t)
+    (inds (inductive_mind ind) (abstract_instance (ind_universes mdecl)) (ind_bodies mdecl)).
+  Proof.
+      Proof.
+    rewrite /inds.
+    induction #|ind_bodies mdecl|; cbn; auto.
+    rtoProp; repeat split; tas.
+    - apply closedq_abstract_instance.
+    - apply closedu_abstract_instance.
+  Qed.
+
+  Lemma wf_ctx_inner_app ui Γ Δ :
+    wf_ctx_inner ui (Γ ,,, Δ) = wf_ctx_inner ui Δ && wf_ctx_inner ui Γ.
+  Proof.
+    apply forallb_app.
+  Qed.
+
+  Lemma wf_ctx_inner_ind_predicate_context {Σ ind mdecl idecl} {wfΣ : wf Σ} :
+    declared_inductive Σ ind mdecl idecl ->
+    closedq_rel #|Instance.qualities (polymorphic_instance (ind_universes mdecl))| idecl.(ind_relevance) ->
+    wf_ctx_inner (polymorphic_instance (ind_universes mdecl)) (ind_params mdecl) ->
+    wf_ctx_inner (polymorphic_instance (ind_universes mdecl)) (ind_indices idecl) ->
+    wf_ctx_inner (abstract_instance (ind_universes mdecl)) (ind_predicate_context ind mdecl idecl).
+  Proof using Type.
+    intros decli.
+    rewrite /ind_predicate_context/=/on_decl_universes/=/on_binder_annot/= ?andb_true_r /closedq_rel /on_relevance => -> /=.
+    rewrite closedq_mkApps closedu_mkApps /=.
+    rewrite closedq_abstract_instance closedu_abstract_instance /= => clpars clinds.
+    have clΓ : wf_ctx_inner (polymorphic_instance (ind_universes mdecl)) (smash_context [] (ind_params mdecl),,, expand_lets_ctx (ind_params mdecl) (ind_indices idecl)).
+    2:repeat (apply/andP; split).
+    - rewrite wf_ctx_inner_app.
+      rewrite wf_ctx_inner_smash_context //.
+      rewrite wf_ctx_inner_expand_lets_ctx //.
+      now rtoProp; split.
+    - apply closedq_to_extended_list_k.
+      by eapply wf_ctx_inner_closedq.
+    - apply closedu_to_extended_list_k.
+      by eapply wf_ctx_inner_closedu.
+    - rewrite wf_ctx_inner_app in clΓ.
+      by rtoProp.
+  Qed.
+
+  Lemma wf_ctx_inner_cstr_branch_context {Σ ind mdecl cdecl} {wfΣ : wf Σ} :
+    wf_ctx_inner (polymorphic_instance (ind_universes mdecl)) (ind_params mdecl) ->
+    wf_ctx_inner (polymorphic_instance (ind_universes mdecl)) (cstr_args cdecl) ->
+    wf_ctx_inner (abstract_instance (ind_universes mdecl)) (cstr_branch_context ind mdecl cdecl).
+  Proof using Type.
+    intros clpars clargs.
+    rewrite /cstr_branch_context.
+    rewrite wf_ctx_inner_expand_lets_ctx // clpars /=.
+    apply wf_ctx_inner_subst_context.
+    rewrite wf_ctx_subst_inds/=.
+    assumption.
+  Qed.
+
+  #[local] Transparent relevance_of_quality.
+  Lemma isSortRel_wf_relevance Σ s r :
+    isSortRel s r ->
+    wf_sort Σ s ->
+    wf_relevance Σ r.
+  Proof.
+    destruct s, r => //= [=] <- [] //.
+  Qed.
+
+  Local Transparent relevance_of_quality.
   Theorem wf_types :
     env_prop (fun Σ Γ t T => wf_universes Σ t && wf_universes Σ T)
-      (fun Σ _ j => lift_wfbu_term (wf_universes Σ) (wf_sortb Σ) j)
+      (fun Σ _ j => lift_wfbu_term (wf_universes Σ) (wf_sortb Σ) (wf_relb Σ) j)
       (fun Σ Γ => wf_ctx_universes Σ Γ).
   Proof using Type.
-    apply typing_ind_env; unfold lift_wfbu_term; intros; rename_all_hyps; cbn; rewrite -!/(wf_universes _ _) ;
+    apply typing_ind_env; unfold lift_wfbu_term; intros; rename_all_hyps;
+    cbn -[wf_qualityb]; rewrite -!/(wf_sortb _ _) -!/(wf_universes _ _) ;
     specIH; to_prop;
-    cbn; auto.
+    cbn -[wf_qualityb]; auto.
 
     - eapply MRReflect.introT. 1: apply lift_wfu_wfbu_term.
-      apply lift_typing_subjtyp with (1 := X) => //= t T [] _ /andP[] //.
+      apply lift_typing_subjtyp with (1 := X) => //=.
+      + move => t T [] _ /andP[] //.
+      + move => t s r [] _ /andP[] _ //= h e.
+        destruct s, r => //=. injection e as [= <-].
+        cbn -[wf_qualityb] in h.
+        rtoProp. assumption.
 
     - apply All_local_env_cst, All_forallb in X0.
-      apply forallb_impl with (2 := X0) => [] [na bo ty] _ //= /andP[] //=.
+      unfold wf_ctx_universes, wf_decl_universes, on_decl_universes.
+      apply forallb_impl with (2 := X0) => [] [na bo ty] _ //= /andP[]/andP[]/andP[] //=.
+      intros; rtoProp; repeat split; tas.
 
     - rewrite wf_universes_lift.
       eapply forallb_nth_error with (n := n) in H0. rewrite heq_nth_error /= in H0.
@@ -1179,41 +1675,36 @@ Section CheckerFlags.
 
     - apply/andP; split; to_wfu; cbn ; eauto with pcuic.
 
-    - cbn in *; to_wfu ; eauto with pcuic.
+    - rtoProp; repeat split; tas.
+      cbn -[wf_qualityb] in *; rewrite -/(wf_sortb _ _) in H3; to_wfu ; eauto with pcuic.
     - rewrite wf_universes_subst. constructor. to_wfu; auto. constructor.
       now move/andP: H1 => [].
 
-    - apply/andP; split.
-      { rewrite wf_universeb_instance_forall andb_comm.
-        apply/wf_instanceP.
-        eapply consistent_instance_ext_wf; eauto. }
-      pose proof (declared_constant_inv _ _ _ _ wf_universes_weaken wf X H0) as [[_ X0]%andb_and _]%andb_and.
+    - apply/andP; split; to_wfu.
+      { eapply consistent_instance_ext_wf; eauto. }
+      pose proof (declared_constant_inv _ _ _ _ wf_universes_weaken wf X H0) as [[[_ X0]%andb_and _]%andb_and _]%andb_and.
       unshelve eapply declared_constant_to_gen in H0; eauto.
       epose proof (weaken_lookup_on_global_env' Σ.1 _ _ wf H0).
       eapply wf_universes_inst. 2:eauto. all:eauto.
       now eapply consistent_instance_ext_wf.
 
-    - apply/andP; split.
-      { rewrite wf_universeb_instance_forall andb_comm.
-        apply/wf_instanceP.
-        eapply consistent_instance_ext_wf; eauto. }
+    - apply/andP; split; to_wfu.
+      { eapply consistent_instance_ext_wf; eauto. }
       pose proof (declared_inductive_inv wf_universes_weaken wf X isdecl).
-      move/onArity : X0 => /andP[] /andP[] /= _ Hind _.
+      move/onArity : X0 => /andP[] /andP[] /= Hind _ _.
       unshelve eapply declared_inductive_to_gen in isdecl; eauto.
       eapply wf_universes_inst; eauto.
       exact (weaken_lookup_on_global_env' Σ.1 _ _ wf (proj1 isdecl)).
       now eapply consistent_instance_ext_wf.
 
-    - apply/andP; split.
-      { rewrite wf_universeb_instance_forall andb_comm.
-        apply/wf_instanceP.
-        eapply consistent_instance_ext_wf; eauto. }
+    - apply/andP; split; to_wfu.
+      { eapply consistent_instance_ext_wf; eauto. }
       pose proof (declared_constructor_inv wf_universes_weaken wf X isdecl) as [sc [nthe onc]].
       unfold type_of_constructor.
       rewrite wf_universes_subst.
       { apply wf_universes_inds.
         now eapply consistent_instance_ext_wf. }
-      move/on_ctype : onc => /andP[] /andP[] /= _ onc _.
+      move/on_ctype : onc => /andP[] /andP[] /= onc _ _.
       clear nthe. unshelve eapply declared_constructor_to_gen in isdecl; eauto.
       eapply wf_universes_inst; eauto.
       exact (weaken_lookup_on_global_env' Σ.1 _ _ wf (proj1 (proj1 isdecl))).
@@ -1223,11 +1714,10 @@ Section CheckerFlags.
       move/andP: H6 => /= [] wfu; rewrite forallb_app.
       move/andP=> [] wfpars wfinds.
       rewrite /wf_universes /on_universes in wfu.
-      move/andP: wfu => [] wfu wfq.
-      rewrite wfu wfq wfpars wf_universes_mkApps /=
+      rewrite wfu wfpars wf_universes_mkApps /=
         forallb_app wfinds /= H0 /= !andb_true_r.
       pose proof (declared_inductive_inv wf_universes_weaken wf X isdecl).
-      move:(onArity X3) => /andP[] /andP[] /= _ hty _.
+      move:(onArity X3) => /andP[] /andP[] /= hty _ _.
       rewrite (ind_arity_eq X3) in hty.
       rewrite !wf_universes_it_mkProd_or_LetIn in hty.
       move/and3P: hty => [] wfp wfindis wfisort.
@@ -1235,38 +1725,38 @@ Section CheckerFlags.
       { eapply (weaken_lookup_on_global_env' _ _ (InductiveDecl mdecl)); eauto.
       unshelve eapply declared_inductive_to_gen in isdecl; eauto.
       }
-      eapply wf_ctx_universes_closed in wfp => //.
-      eapply wf_ctx_universes_closed in wfindis => //.
-      rewrite (consistent_instance_univs_length H2).
-      erewrite closedu_compare_decls; tea.
-      rewrite closed_ind_predicate_context // /=.
-      unfold test_branch.
-      apply/andP; split.
-      * have wfbrctx : All (fun cdecl =>
-          closedu_ctx #|Instance.universes (polymorphic_instance (ind_universes mdecl))| (cstr_args cdecl))
-          (ind_ctors idecl).
+      eapply wf_ctx_universes_inner in wfp => //.
+      eapply wf_ctx_universes_inner in wfindis => //.
+      rtoProp; repeat split.
+      * cbn in H8. to_wfu.
+        eapply isSortRel_wf_relevance; tea.
+      * erewrite wf_ctx_inner_compare_decls; tea.
+        erewrite wf_ctx_inner_lengths.
+        1: apply wf_ctx_inner_ind_predicate_context; eauto.
+        + cbn -[wf_qualityb] in wfisort. to_wfu.
+          eapply wf_relevance_closed.
+          eapply isSortRel_wf_relevance; tea.
+          apply X3.
+        + apply (consistent_instance_quals_length H2).
+        + apply (consistent_instance_univs_length H2).
+      * have wfbrctx : All (fun cdecl => wf_ctx_inner (polymorphic_instance (ind_universes mdecl)) (cstr_args cdecl)) (ind_ctors idecl).
         { pose proof (onConstructors := onConstructors X3).
           clear -wf ond onConstructors.
           red in onConstructors. solve_all. destruct X.
-          move : on_ctype => /andP[] /andP[] /= _ wfty _.
+          move : on_ctype => /andP[] /andP[] /= wfty _ _.
           rewrite cstr_eq in wfty.
           rewrite !wf_universes_it_mkProd_or_LetIn in wfty.
           move/and3P: wfty => [] _ clargs _.
-          apply wf_ctx_universes_closed in clargs => //. }
+          apply wf_ctx_universes_inner in clargs => //. }
         solve_all.
-        erewrite closedu_compare_decls; [|tea].
-        rewrite /cstr_branch_context.
-        eapply closedu_expand_lets_ctx.
-        rewrite wfp. eapply closedu_subst_context.
-        rewrite a.
-        now rewrite closedu_inds.
+        erewrite wf_ctx_inner_compare_decls; [|tea].
+        erewrite wf_ctx_inner_lengths.
+        1:apply wf_ctx_inner_cstr_branch_context; tas.
+        + apply (consistent_instance_quals_length H2).
+        + apply (consistent_instance_univs_length H2).
       * rewrite wf_universes_it_mkLambda_or_LetIn H7 andb_true_r.
         move: H4.
-        rewrite /wf_ctx_universes forallb_app => /andP[hctx _].
-        apply (MRReflect.introT onctxP).
-        solve_all. unfold ondecl, wf_decl_universes, on_decl_universes in *.
-        move/andP:H3 => [Hb Ht] //; split; tas.
-        now destruct decl_body.
+        rewrite /wf_ctx_universes forallb_app => /andP[hctx _] //.
 
     - rewrite /subst1. rewrite wf_universes_subst.
       constructor => //. eapply All_rev.
@@ -1281,11 +1771,9 @@ Section CheckerFlags.
       red in o0.
       destruct nth_error eqn:heq => //.
       destruct o0  as [_ ->].
-      rewrite wf_universes_mkApps {1}/wf_universes /= -!/(wf_universes _ _)
-        wf_universeb_instance_forall in H2.
+      rewrite wf_universes_mkApps {1}/wf_universes /= -!/(wf_universes _ _) in H2.
       move/andP: H2 => [wfu wfargs].
-      rewrite andb_comm in wfu.
-      move/wf_instanceP: wfu => wfu.
+      move/on_instance_reflect: wfu => wfu.
       unshelve eapply declared_projection_to_gen in isdecl; eauto.
       eapply (wf_universes_inst (ind_universes mdecl)); eauto.
       exact (weaken_lookup_on_global_env' Σ.1 _ _ wf (proj1 (proj1 (proj1 isdecl)))).
@@ -1307,7 +1795,7 @@ Section CheckerFlags.
       noconf heq. simpl.
       rewrite wf_universes_subst.
       apply wf_extended_subst.
-      rewrite ind_arity_eq in onArity. move:onArity => /andP[] /andP[] /= _ Hs _.
+      rewrite ind_arity_eq in onArity. move:onArity => /andP[] /andP[] /= Hs _ _.
       rewrite !wf_universes_it_mkProd_or_LetIn in Hs.
       now move/andP: Hs => /andP /andP [].
       rewrite wf_universes_lift.
@@ -1317,12 +1805,12 @@ Section CheckerFlags.
     - clear X X1. unfold on_def_type, on_def_body in *; cbn in *.
       apply/andP; split; auto.
       solve_all.
-      eapply nth_error_all in X0 as (? & _)%andb_and; eauto.
+      eapply nth_error_all in X0 as ((? & _)%andb_and & _)%andb_and; eauto.
 
     - clear X X1. unfold on_def_type, on_def_body in *; cbn in *.
       apply/andP; split; auto.
       solve_all.
-      eapply nth_error_all in X0 as (? & _)%andb_and; eauto.
+      eapply nth_error_all in X0 as ((? & _)%andb_and & _)%andb_and; eauto.
 
     - apply/andP; split; eauto.
       destruct X0; cbn => //.
@@ -1339,13 +1827,22 @@ Qed.
     exact (env_prop_typing wf_types _ wfΣ _ _ _ Hty).
   Qed.
 
+  Lemma typing_wf_ctx_universes {Σ : global_env_ext} {Γ} :
+    wf Σ ->
+    wf_local Σ Γ ->
+    wf_ctx_universes Σ Γ.
+  Proof using Type.
+    intros wfΣ Hty.
+    by apply (env_prop_wf_local wf_types).
+  Qed.
+
   Lemma typing_wf_sort {Σ : global_env_ext} {Γ t s} :
     wf Σ ->
     Σ ;;; Γ |- t : tSort s -> wf_sort Σ s.
   Proof using Type.
     intros wfΣ Hty.
     apply typing_wf_universes in Hty as [_ wfs]%andb_and; auto.
-    cbn in wfs. now to_wfu.
+    cbn -[wf_qualityb] in wfs. rewrite -/(wf_sortb _ s) in wfs. now to_wfu.
   Qed.
 
   Lemma isType_wf_universes {Σ Γ T} : wf Σ.1 -> isType Σ Γ T -> wf_universes Σ T.
@@ -1362,3 +1859,473 @@ Hint Extern 4 (wf_sort _ ?u) =>
   match goal with
   [ H : typing _ _ _ (tSort u) |- _ ] => apply (typing_wf_sort _ H)
   end : pcuic.
+
+
+
+From Stdlib Require Import Morphisms.
+From Stdlib Require Import ssreflect.
+Set SimplIsCbn.
+
+Section SubstIdentity.
+  Context `{cf:checker_flags}.
+
+  Lemma subst_instance_level_abs l n Σ qs :
+    wf Σ ->
+    LevelSet.In l (LevelSet.union
+     (fold_right LevelSet.add LevelSet.empty
+        (unfold n Level.lvar)) (global_levels Σ)) ->
+    subst_instance_level (Instance.make qs (unfold n Level.lvar)) l = l.
+  Proof using Type.
+    intros wfΣ lin.
+    eapply LevelSet.union_spec in lin.
+    destruct lin.
+    - apply LevelSet_In_fold_right_add in H.
+      destruct l; simpl; auto.
+      eapply In_unfold_inj in H; [|congruence].
+      pose proof (proj1 (nth_error_unfold Level.lvar n n0) H).
+      now rewrite (nth_error_nth _ _ _ H0).
+    - eapply not_var_global_levels in wfΣ.
+      specialize (wfΣ l H). simpl in wfΣ.
+      destruct l => //.
+  Qed.
+
+  Lemma consistent_instance_ext_abstract_instance Σ udecl :
+    wf Σ ->
+    wf_global_ext Σ udecl ->
+    consistent_instance_ext (Σ, udecl) udecl (abstract_instance udecl).
+  Proof using Type.
+    intros wfΣ wf_glob_ext.
+    red. red.
+    destruct udecl as [|[univs cst]] eqn:indu.
+    { simpl; split; reflexivity. }
+    repeat split.
+    - simpl abstract_instance. eapply forallb_mapi => //.
+      intros i Hi. unfold global_ext_qualities.
+      apply QualitySet.mem_spec, QualitySet.union_spec. left.
+      unfold qualities_of_udecl. simpl.
+      rewrite (mapi_unfold Quality.var). eapply QualitySet_In_fold_right_add.
+      induction #|qualities univs| in i, Hi |- *; try lia.
+      simpl. eapply in_or_app. destruct (eq_dec i n).
+      * subst. right; simpl; auto.
+      * left; apply IHn; lia.
+    - now rewrite mapi_length.
+    - simpl abstract_instance.
+      eapply forallb_mapi => //.
+      intros i Hi. unfold global_ext_levels.
+      apply LevelSet.mem_spec, LevelSet.union_spec. left.
+      unfold levels_of_udecl. simpl.
+      rewrite (mapi_unfold Level.lvar).
+      eapply LevelSet_In_fold_right_add.
+      induction #|Universes.universes univs| in i, Hi |- *; try lia.
+      simpl. eapply in_or_app. destruct (eq_dec i n).
+      * subst. right; simpl; auto.
+      * left; apply IHn; lia.
+    - now rewrite mapi_length.
+    - simpl. rewrite (mapi_unfold Level.lvar).
+      assert(CS.Equal (subst_instance_cstrs (Instance.make (mapi (fun (i : nat) (_ : name) => Quality.var i) (qualities univs)) (unfold #|Universes.universes univs| Level.lvar)) cst) cst).
+      { unfold CS.Equal; intros a.
+        unfold subst_instance_cstrs.
+        red in wf_glob_ext.
+        destruct wf_glob_ext as [_ wfext].
+        unfold on_udecl_prop in wfext.
+        simpl constraints_of_udecl in wfext.
+        simpl levels_of_udecl in wfext.
+        rewrite (mapi_unfold Level.lvar) in wfext.
+        clear indu.
+        simpl fst in wfext.
+        revert wfext.
+        eapply ConstraintSetProp.fold_rec_weak; auto.
+        2:reflexivity.
+        * intros s s' a' eqs H.
+          intros Hf.
+          rewrite <- eqs in Hf. rewrite -eqs; auto.
+        * intros x a0 s nin equiv.
+          intros cadd.
+          eapply CS_For_all_add in cadd as [cadd Ps].
+          specialize (equiv Ps). clear Ps.
+          destruct x as [[l c] r]. destruct cadd as [inl inr].
+          unfold subst_instance_cstr. simpl.
+          eapply subst_instance_level_abs with (qs := (mapi (fun (i : nat) (_ : name) => Quality.var i) (qualities univs))) in inl; auto.
+          eapply subst_instance_level_abs with (qs := (mapi (fun (i : nat) (_ : name) => Quality.var i) (qualities univs))) in inr; auto.
+          rewrite inl inr.
+          rewrite !CS.add_spec.
+          intuition auto. }
+      unfold valid_constraints. destruct check_univs; auto.
+      unfold valid_constraints0, satisfies. intros v.
+      destruct univs. cbn in *. rewrite H.
+      eapply CS_For_all_union.
+  Qed.
+
+  Lemma global_level_subst_abs Σ u :
+    wf_ext_wk Σ ->
+    LevelSet.In u (global_ext_levels Σ) ->
+    subst_instance_level (abstract_instance Σ.2) u = u.
+  Proof using Type.
+    intros [wfΣ onu] declu.
+    destruct u; simpl; auto. cbn -[global_ext_levels] in declu.
+    eapply in_var_global_ext in declu; auto.
+    destruct (udecl_prop_in_var_poly declu) as [[univs csts] eq].
+    rewrite eq in declu |- *. simpl in *.
+    rewrite mapi_unfold in declu |- *.
+    eapply LevelSet_In_fold_right_add in declu.
+    eapply In_unfold_inj in declu; try congruence.
+    eapply (nth_error_unfold Level.lvar) in declu.
+    now rewrite (nth_error_nth _ _ _ declu).
+  Qed.
+
+  Lemma wf_qvar_subst_abs Σ qv :
+    wf_qvar Σ qv ->
+    subst_instance_qvar (abstract_instance Σ.2) qv = Quality.qVar qv.
+  Proof using Type.
+    intros declq.
+    cbn -[global_ext_qualities] in declq.
+    destruct qv.
+    eapply in_var_global_ext' in declq; auto.
+    destruct (udecl_in_var_quality_poly declq) as [[univs csts] eq].
+    rewrite eq in declq |- *. simpl in *.
+    rewrite mapi_unfold in declq |- *.
+    eapply QualitySet_In_fold_right_add in declq.
+    eapply In_unfold_inj in declq.
+    2: intros ?? H; injection H => //.
+    eapply (nth_error_unfold Quality.var) in declq.
+    now rewrite (nth_error_nth _ _ _ declq).
+  Qed.
+
+  Lemma wf_quality_subst_abs Σ q :
+    wf_quality Σ q ->
+    subst_instance_quality (abstract_instance Σ.2) q = q.
+  Proof using Type.
+    intros declq.
+    destruct q; simpl; auto.
+    apply wf_qvar_subst_abs; auto.
+  Qed.
+(*
+  Lemma consistent_instance_ext_subst_abs Σ decl u :
+    wf_ext_wk Σ ->
+    consistent_instance_ext Σ decl u ->
+    subst_instance (abstract_instance Σ.2) u = u.
+  Proof using Type.
+    intros wfΣ cu.
+    destruct decl.
+    { simpl in cu. destruct u, cu; simpl in *.
+      apply length_nil in H, H0. rewrite H H0 //. }
+    destruct u as [qs us].
+    rewrite /subst_instance /subst_instance_instance // /Instance.make /=.
+    destruct cu as (hq & _ & hl & _).
+    cbn -[QualitySet.mem LS.mem] in *.
+    apply forallb_All in hq, hl.
+    f_equal; eapply All_map_id, All_impl; eauto; cbn -[QualitySet.mem LS.mem]; intros.
+    - eapply wf_quality_subst_abs; tea.
+      now apply QualitySet.mem_spec.
+    - eapply global_level_subst_abs; tea.
+      now apply LS.mem_spec.
+  Qed. *)
+
+  Lemma wf_instance_subst_abs Σ u :
+    wf_ext_wk Σ ->
+    wf_instance Σ u ->
+    subst_instance (abstract_instance Σ.2) u = u.
+  Proof using Type.
+    intros wfΣ cu.
+    destruct u as [qs us].
+    rewrite /subst_instance /subst_instance_instance // /Instance.make /=.
+    destruct cu; cbn in *.
+    f_equal; solve_all.
+    - by apply wf_quality_subst_abs.
+    - by apply global_level_subst_abs.
+  Qed.
+
+  Lemma in_global_ext_subst_abs_level Σ l :
+    wf_ext_wk Σ ->
+    LevelSet.In (LevelExpr.get_level l) (global_ext_levels Σ) ->
+    subst_instance (abstract_instance Σ.2) l = l.
+  Proof using Type.
+    intros wfΣ cu.
+    destruct l; auto.
+    apply global_level_subst_abs in cu; tea.
+    cbn in cu.
+    destruct t; cbn; auto.
+    rewrite /= nth_nth_error in cu.
+    destruct nth_error => //. congruence.
+  Qed.
+
+  Lemma wf_universe_subst_abs Σ u :
+    wf_ext_wk Σ ->
+    wf_universe Σ u ->
+    subst_instance_universe (abstract_instance Σ.2) u = u.
+  Proof using Type.
+    intros wf cu.
+    simpl in cu.
+    apply NonEmptySetFacts.eq_univ'.
+    intros l.
+    rewrite In_subst_instance.
+    split.
+    - intros [x [inx ->]].
+      specialize (cu _ inx).
+      unfold subst_instance.
+      apply in_global_ext_subst_abs_level in cu; eauto.
+      unfold subst_instance in cu. now rewrite cu.
+    - intros inl.
+      specialize (cu _ inl). exists l; split; auto.
+      now rewrite in_global_ext_subst_abs_level.
+  Qed.
+
+  Lemma wf_sort_subst_abs Σ u :
+    wf_ext_wk Σ ->
+    wf_sort Σ u ->
+    subst_instance_sort (abstract_instance Σ.2) u = u.
+  Proof using Type.
+    intros wf cu.
+    destruct u; simpl; auto.
+    - f_equal.
+      by apply wf_universe_subst_abs.
+    - destruct cu as [hq hl].
+      eapply wf_qvar_subst_abs in hq as ->; tea.
+      eapply wf_universe_subst_abs in hl; tea.
+      rewrite /subst_instance hl //.
+  Qed.
+
+  (* Lemma consistent_instance_ext_subst_abs_inds Σ decl ind u bodies :
+    wf_ext_wk Σ ->
+    consistent_instance_ext Σ decl u ->
+    subst_instance (abstract_instance Σ.2) (inds ind u bodies) =
+      (inds ind u bodies).
+  Proof using Type.
+    intros wf cu.
+    unfold inds. generalize #|bodies|.
+    induction n; simpl; auto. rewrite IHn; f_equal.
+    now rewrite [subst_instance_instance _ _](consistent_instance_ext_subst_abs _ _ _ wf cu).
+  Qed. *)
+
+  Lemma wf_relevance_subst_abs Σ r :
+    wf_ext_wk Σ ->
+    wf_relevance Σ r ->
+    subst_instance (abstract_instance Σ.2) r = r.
+  Proof using Type.
+    intros wf cu.
+    unfold subst_instance, subst_instance_aname, subst_instance_binder_annot.
+    destruct r => //=. cbn in cu.
+    rewrite wf_qvar_subst_abs //.
+  Qed.
+
+  Lemma wf_relevance_subst_abs_aname Σ na :
+    wf_ext_wk Σ ->
+    wf_relevance Σ na.(binder_relevance) ->
+    subst_instance (abstract_instance Σ.2) na = na.
+  Proof using Type.
+    intros wf cu.
+    unfold subst_instance, subst_instance_aname, subst_instance_binder_annot.
+    destruct na as [n r]; f_equal; cbn in *.
+    by apply wf_relevance_subst_abs.
+  Qed.
+
+  Lemma app_inj {A} (l l' l0 l0' : list A) :
+    #|l| = #|l0| ->
+    l ++ l' = l0 ++ l0' ->
+    l = l0 /\ l' = l0'.
+  Proof using Type.
+    induction l in l', l0, l0' |- *; destruct l0; simpl in * => //; auto.
+    intros [= eq] [= -> eql].
+    now destruct (IHl _ _ _ eq eql).
+  Qed.
+
+  Ltac to_wfu :=
+    repeat match goal with
+    | [ H: is_true (wf_qualityb _ ?x) |- _ ] => apply (elimT (@wf_qualityP _ x)) in H
+    | [ |- is_true (wf_qualityb _ ?x) ] => apply (introT (@wf_qualityP _ x))
+    | [ H: is_true (wf_universeb _ ?x) |- _ ] => apply (elimT (@wf_universe_reflect _ x)) in H
+    | [ |- is_true (wf_universeb _ ?x) ] => apply (introT (@wf_universe_reflect _ x))
+    | [ H: is_true (Sort.on_sort _ (wf_universeb _) _ _ ?x) |- _ ] => apply (elimT (@wf_sort_reflect _ x)) in H
+    | [ |- is_true (Sort.on_sort _ (wf_universeb _) _ _ ?x) ] => apply (introT (@wf_sort_reflect _ x))
+    | [ H: is_true (wf_sortb _ ?x) |- _ ] => apply (elimT (@wf_sort_reflect _ x)) in H
+    | [ |- is_true (wf_sortb _ ?x) ] => apply (introT (@wf_sort_reflect _ x))
+    | [ H: is_true (on_instance (wf_qualityb _) (wf_universeb _) ?x) |- _ ] => apply (elimT (@on_instance_reflect _ x)) in H
+    | [ |- is_true (on_instance (wf_qualityb _) (wf_universeb _) ?x) ] => apply (introT (@on_instance_reflect _ x))
+    | [ H: is_true (on_relevance _ _ ?x) |- _ ] => apply (elimT (@on_relevance_reflect _ x)) in H
+    | [ |- is_true (on_relevance _ _ ?x) ] => apply (introT (@on_relevance_reflect _ x))
+    | [ H: is_true (on_binder_annot _ ?x) |- _ ] => apply (elimT (@on_binder_annot_reflect _ x)) in H
+    | [ |- is_true (on_binder_annot _ ?x) ] => apply (introT (@on_binder_annot_reflect _ x))
+    end.
+
+  Lemma subst_abstract_instance_id Σ t :
+    wf_ext_wk Σ ->
+    wf_universes Σ t ->
+    let u := abstract_instance (snd Σ) in
+    t@[u] = t.
+  Proof.
+    intros wfΣ h.
+    induction t in h |- * using term_forall_list_ind.
+    all: cbn -[Universe.make' wf_qualityb] in *; auto.
+    all: rtoProp; to_wfu.
+    all: try solve [ f_equal; solve_all; to_wfu; eauto using wf_relevance_subst_abs_aname, wf_instance_subst_abs, wf_sort_subst_abs ].
+    - f_equal; auto.
+      + unfold map_case_info.
+        destruct ci; cbn; f_equal.
+        destruct ci_relevance => //.
+        by apply wf_relevance_subst_abs.
+      + unfold map_predicate.
+        destruct p; cbn in *; f_equal; solve_all.
+        by apply wf_instance_subst_abs.
+      + solve_all.
+    - f_equal.
+      destruct p as [? []]; cbnr.
+      cbn -[Universe.make'] in X, h. do 2 f_equal.
+      unfold mapu_array_model.
+      rtoProp. to_wfu. destruct X as (?&?&?).
+      destruct a; cbn -[Universe.make'] in *; f_equal; eauto.
+      + apply global_level_subst_abs; tas.
+        by apply wf_universe_make.
+      + solve_all.
+  Qed.
+
+  Lemma subst_context_abstract_instance_id Σ Γ :
+    wf_ext_wk Σ ->
+    wf_ctx_universes Σ Γ ->
+    let u := abstract_instance (snd Σ) in
+    Γ@[u] = Γ.
+  Proof.
+    unfold subst_instance, subst_instance_context, map_context_gen, map_decl_gen, wf_ctx_universes.
+    solve_all.
+    move: H => /andP[]/andP[] hna hb hty.
+    destruct x; cbn -[wf_qualityb] in *; f_equal.
+    - to_wfu.
+      by apply wf_relevance_subst_abs_aname.
+    - destruct decl_body; cbnr. f_equal.
+      by apply subst_abstract_instance_id.
+    - by apply subst_abstract_instance_id.
+  Qed.
+
+(*
+  Lemma subst_abstract_instance_id :
+    env_prop (fun Σ Γ t T =>
+        wf_ext_wk Σ ->
+        let u := abstract_instance (snd Σ) in
+        subst_instance u t = t × subst_instance u T = T)
+        (fun Σ _ j => wf_ext_wk Σ ->
+        let u := abstract_instance (snd Σ) in
+        lift_wfu_term (fun t => subst_instance u t = t) (fun u => wf_sort Σ u) j)
+        (fun Σ Γ =>
+        wf_ext_wk Σ ->
+        let u := abstract_instance (snd Σ) in
+        subst_instance u Γ = Γ).
+  Proof using Type.
+
+    eapply typing_ind_env; intros; simpl in *; auto.
+    { apply lift_typing_subjtyp with (1 := X). 2: intros s Hs; now depelim Hs.
+      intros ?? []; auto. }
+
+    { apply All_local_env_cst in X0. clear -X0 X1.
+      eapply All2_eq, All2_map_left. apply All_All2 with (1 := X0) => decl IH.
+      destruct IH as (? & ? & ?), decl as [na bo ty]; tas; unfold map_decl; cbn in *.
+      f_equal; tas. destruct bo => //. all: admit. cbn in *. now f_equal. }
+
+    all: try ((subst u || subst u0); split; [f_equal|]; intuition eauto).
+
+    1:{ rewrite subst_instance_lift. f_equal.
+      generalize H. rewrite -H1 /subst_instance /= nth_error_map H /= => [=].
+      intros Hdecl. now rewrite -{2}Hdecl. }
+
+    all: try match goal with H : lift_wfu_term _ _ _ |- _ => destruct H as (Htm & Hty & Hs); cbn in Htm, Hty, Hs end.
+    all:try (solve [f_equal; eauto; try congruence]).
+    all:try (rewrite ?subst_instance_two; f_equal; eapply consistent_instance_ext_subst_abs; eauto).
+
+    - now rewrite wf_sort_subst_abs.
+
+    - rewrite wf_sort_subst_abs //.
+      now apply wf_sort_super.
+
+    - rewrite product_subst_instance. do 2 f_equal; tas.
+      now noconf b0.
+
+    - intuition auto. noconf a; noconf b; noconf b0.
+      rewrite subst_instance_subst /= /subst1.
+      repeat (f_equal; simpl; auto).
+
+    - rewrite /type_of_constructor subst_instance_subst subst_instance_two.
+      erewrite consistent_instance_ext_subst_abs; eauto. f_equal.
+      eapply consistent_instance_ext_subst_abs_inds; eauto.
+
+    - solve_all; simpl in *.
+      * rewrite subst_instance_mkApps /= /subst_instance /= in b0.
+        eapply mkApps_nApp_inj in b0 as [Hi Hpars] => //.
+        now noconf Hi.
+      * rewrite subst_instance_mkApps /= /subst_instance /= in b0.
+        eapply mkApps_nApp_inj in b0 as [Hi Hpars] => //.
+        rewrite map_app in Hpars.
+        eapply app_inj in Hpars as [Hpars hinds]. 2:now len.
+        rewrite -{2}(map_id (pparams p)) in Hpars.
+        now apply map_eq_inj in Hpars.
+
+    - solve_all.
+
+    - rewrite subst_instance_mkApps. f_equal.
+      * rewrite /ptm.
+        rewrite subst_instance_it_mkLambda_or_LetIn.
+        rewrite subst_instance_app in H.
+        eapply app_inj in H as []; [|now len].
+        rewrite H. now f_equal.
+      * rewrite map_app.
+        rewrite subst_instance_mkApps /= /subst_instance /= in b0.
+        eapply mkApps_nApp_inj in b0 as [Hi Hpars] => //.
+        rewrite map_app in Hpars.
+        eapply app_inj in Hpars as [Hpars hinds]. 2:now len.
+        now rewrite hinds /= a0.
+    - rewrite subst_instance_subst /=.
+      rewrite /subst_instance /=.
+      rewrite subst_instance_mkApps in b.
+      eapply mkApps_nApp_inj in b as [Hi Hpars] => //.
+      f_equal.
+      * rewrite a; f_equal.
+        rewrite /subst_instance_list. now rewrite map_rev Hpars.
+      * rewrite [subst_instance_constr _ _]subst_instance_two.
+        noconf Hi. now rewrite [subst_instance _ u]H.
+    - solve_all.
+      + destruct a0 as (_ & X & _); tas.
+      + destruct b as (X & _); tas.
+    - eapply nth_error_all in X0 as (_ & X0 & _); tea.
+    - solve_all.
+      + destruct a0 as (_ & X & _); tas.
+      + destruct b as (X & _); tas.
+    - eapply nth_error_all in X0 as (_ & X0 & _); tea.
+    - destruct p as [? []]; cbnr. do 2 f_equal.
+      depelim X0. specialize (hty X1); specialize (hdef X1).
+      unfold mapu_array_model; destruct a; cbn -[Universe.make'] in *.
+      f_equal; intuition eauto.
+      * rewrite /subst_instance subst_instance_universe_make in b.
+        now injection b as e.
+      * solve_all.
+    - depelim X0; cbn => //=. depelim X. simp prim_type. cbn. f_equal; intuition eauto.
+      do 2 f_equal.
+      cbn -[Universe.make'] in b.
+      rewrite /subst_instance subst_instance_universe_make in b.
+      injection b as e. unfold subst_instance_instance. cbn; f_equal.
+      now unfold subst_instance in e.
+  Qed. *)
+
+  Lemma typed_subst_abstract_instance Σ Γ t T :
+    wf_ext_wk Σ ->
+    Σ ;;; Γ |- t : T ->
+    let u := abstract_instance Σ.2 in
+    subst_instance u t = t.
+  Proof using Type.
+    intros wfΣ H.
+    apply subst_abstract_instance_id; tas.
+    apply typing_wf_universes in H as (?&?)%andb_and; tas.
+    apply wfΣ.
+  Qed.
+
+  Lemma subst_instance_id Σ Γ :
+    wf_ext_wk Σ ->
+    wf_local Σ Γ ->
+    let u := abstract_instance Σ.2 in
+    subst_instance u Γ = Γ.
+  Proof using Type.
+    intros wfΣ H.
+    eapply subst_context_abstract_instance_id; tas.
+    apply typing_wf_ctx_universes; tas.
+    apply wfΣ.
+  Qed.
+
+End SubstIdentity.
+
+Hint Resolve declared_inductive_wf_ext_wk declared_inductive_wf_global_ext : pcuic.
