pcuic/theories/Syntax/PCUICCases.v
@@ -91,7 +91,7 @@ Definition case_predicate_context_gen ind mdecl idecl params puinst pctx :=
   map2 set_binder_name pctx (pre_case_predicate_context_gen ind mdecl idecl params puinst).
 
 Definition case_predicate_context ind mdecl idecl p : context :=
-  case_predicate_context_gen ind mdecl idecl p.(pparams) p.(puinst) (forget_types p.(pcontext)).
+  case_predicate_context_gen ind mdecl idecl p.(pparams) p.(puinst) (forget_types p.(pcontext))@[p.(puinst)].
 Arguments case_predicate_context _ _ _ !_.
 
 Definition cstr_branch_context ind mdecl cdecl : context :=
@@ -121,7 +121,7 @@ Definition case_branch_context_gen ind mdecl params puinst pctx cdecl :=
   map2 set_binder_name pctx (pre_case_branch_context_gen ind mdecl cdecl params puinst).
 
 Definition case_branch_context ind mdecl p bctx cdecl : context :=
-  case_branch_context_gen ind mdecl p.(pparams) p.(puinst) bctx cdecl.
+  case_branch_context_gen ind mdecl p.(pparams) p.(puinst) bctx@[p.(puinst)] cdecl.
 Arguments case_branch_context _ _ _ !_.
 (*
 Definition case_branch_context_gen ind mdecl params puinst bctx cdecl : context :=
@@ -159,7 +159,7 @@ Definition case_branch_type_gen ind mdecl (idecl : one_inductive_body) params pu
   (brctx, ty).
 
 Definition case_branch_type ind mdecl idecl p (b : branch term) ptm i cdecl : context * term :=
-  case_branch_type_gen ind mdecl idecl p.(pparams) p.(puinst) (forget_types b.(bcontext)) ptm i cdecl.
+  case_branch_type_gen ind mdecl idecl p.(pparams) p.(puinst) (forget_types b.(bcontext))@[p.(puinst)] ptm i cdecl.
 Arguments case_branch_type _ _ _ _ _ _ _ !_.
 
 Lemma case_branch_type_fst ci mdecl idecl p br ptm c cdecl :
@@ -260,9 +260,8 @@ Lemma case_predicate_context_length {ci mdecl idecl p} :
   #|case_predicate_context (ci_ind ci) mdecl idecl p| = #|p.(pcontext)|.
 Proof.
   intros hl.
-  unfold case_predicate_context, case_predicate_context_gen, pre_case_predicate_context_gen.
-  rewrite map2_length /= //.
-  2:len => //.
+  unfold case_predicate_context, case_predicate_context_gen, pre_case_predicate_context_gen, subst_instance, subst_instance_list.
+  rewrite map2_length length_map /= //. 2: by rewrite length_map //.
   destruct hl.
   rewrite (Forall2_length H0). len. now len.
 Qed.
@@ -272,12 +271,9 @@ Lemma case_predicate_context_length_indices {ci mdecl idecl p} :
   #|case_predicate_context (ci_ind ci) mdecl idecl p| = S #|idecl.(ind_indices)|.
 Proof.
   intros hl.
-  unfold case_predicate_context, case_predicate_context_gen, pre_case_predicate_context_gen.
+  rewrite case_predicate_context_length //.
   pose proof (Forall2_length (proj2 hl)). simpl in H.
-  rewrite -H.
-  rewrite map2_length; len. all:len.
-  - now len in H.
-  - now len in H.
+  rewrite length_map // in H.
 Qed.
 
 Lemma wf_predicate_length_pars {mdecl idecl p} :
@@ -305,11 +301,10 @@ Lemma case_branch_context_length {ind mdecl p br cdecl} :
   #|case_branch_context ind mdecl p (forget_types br.(bcontext)) cdecl| = #|br.(bcontext)|.
 Proof.
   intros hl.
-  unfold case_branch_context, case_branch_context_gen, pre_case_branch_context_gen; len.
-  rewrite map2_length //.
-  * red in hl. red in hl.
-    rewrite (Forall2_length hl). now len.
-  * now len.
+  unfold case_branch_context, case_branch_context_gen, pre_case_branch_context_gen, subst_instance, subst_instance_list.
+  rewrite map2_length length_map /= //. 2: by rewrite length_map //.
+  do 2 red in hl.
+  rewrite (Forall2_length hl). now len.
 Qed.
 
 Lemma case_branch_context_length_args {ind mdecl p br cdecl} :
@@ -317,9 +312,9 @@ Lemma case_branch_context_length_args {ind mdecl p br cdecl} :
   #|case_branch_context ind mdecl p (forget_types br.(bcontext)) cdecl| = #|cdecl.(cstr_args)|.
 Proof.
   intros hl.
-  unfold case_branch_context, case_branch_context_gen, pre_case_branch_context_gen; len.
-  apply Forall2_length in hl.
-  rewrite map2_length //. rewrite hl. now len.
+  apply Forall2_length in hl as h.
+  apply case_branch_context_length in hl as ->.
+  rewrite -h length_map //.
 Qed.
 
 Lemma case_branch_context_assumptions {ind mdecl p br cdecl} :
@@ -328,11 +323,10 @@ Lemma case_branch_context_assumptions {ind mdecl p br cdecl} :
   context_assumptions cdecl.(cstr_args).
 Proof.
   intros hl.
-  unfold case_branch_context, case_branch_context_gen, pre_case_branch_context_gen; len.
+  unfold case_branch_context, case_branch_context_gen, pre_case_branch_context_gen, subst_instance, subst_instance_list; len.
   apply Forall2_length in hl.
-  rewrite /expand_lets_ctx /expand_lets_k_ctx. len.
   rewrite map2_set_binder_name_context_assumptions.
-  - now rewrite hl; len.
+  - now rewrite length_map hl; len.
   - len. rewrite /cstr_branch_context /expand_lets_ctx /expand_lets_k_ctx. now len.
 Qed.
 
